\newpage
\subsection{Exercise 26.1}
\begin{enumerate}
      \begin{multicols}{2}
            \item Find the equations of the tangent and normal to the curve $y = x^2 + 2$ at
            point $(2, 6)$. \sol{}
            \begin{flalign*}
                  y              & = x^2 + 2 & \\
                  \dfrac{dy}{dx} & = 2x
            \end{flalign*}
            At point $(2, 6)$,
            \begin{flalign*}
                  \text{Gradient of tangent } \dfrac{dy}{dx} & = 2(2) = 4      & \\
                  \text{Gradient of normal }                 & = -\dfrac{1}{4}
            \end{flalign*}
            \begin{flalign*}
                  \therefore\ \text{Equation of tangent is } y - 6 & = 4(x - 2)             & \\
                  y                                                & = 4x - 2               & \\
                  \text{Equation of normal is } y - 6              & = -\dfrac{1}{4}(x - 2) & \\
                  4y - 24                                          & = -x + 2               & \\
                  x + 4y                                           & = 26
            \end{flalign*}

            \item Find the equation of the tangent to the curve $y = 2x^3 - 3x^2 - 12x + 8$ where
            $x = 0$. \sol{}
            \begin{flalign*}
                  y              & = 2x^3 - 3x^2 - 12x + 8 & \\
                  \dfrac{dy}{dx} & = 6x^2 - 6x - 12
            \end{flalign*}
            At $x = 0$, $y = 8$
            \begin{flalign*}
                  \text{Gradient of tangent } \dfrac{dy}{dx}       & = 6(0)^2 - 6(0) - 12 = -12 & \\
                  \therefore\ \text{Equation of tangent is } y - 8 & = -12(x - 0)               & \\
                  y                                                & = -12x + 8
            \end{flalign*}
      \end{multicols}
      \vfill\null

      \begin{multicols}{2}
            \item Find the equation of the normal to the curve $y = 3x^3 - 4x + 7$ at point $(1,
                  6)$. \sol{}
            \begin{flalign*}
                  y              & = 3x^3 - 4x + 7 & \\
                  \dfrac{dy}{dx} & = 9x^2 - 4
            \end{flalign*}
            At point $(1, 6)$,
            \begin{flalign*}
                  \text{Gradient of tangent } \dfrac{dy}{dx} & = 9(1)^2 - 4 = 5 & \\
                  \text{Gradient of normal }                 & = -\dfrac{1}{5}
            \end{flalign*}
            \begin{flalign*}
                  \therefore\ \text{Equation of normal is } y - 6 & = -\dfrac{1}{5}(x - 1) & \\
                  5y - 30                                         & = -x + 1               & \\
                  x + 5y                                          & = 31
            \end{flalign*}

            \item Find the equation of the tangent to the curve $y = \dfrac{1}{1-x}$ where $x =
                  -1$. \sol{}
            \begin{flalign*}
                  y              & = \dfrac{1}{1-x}     & \\
                  \dfrac{dy}{dx} & = \dfrac{1}{(1-x)^2}
            \end{flalign*}
            At $x = -1$, $y = \dfrac{1}{2}$
            \begin{flalign*}
                  \text{Gradient of tangent } \dfrac{dy}{dx}                  & = \dfrac{1}{[1-(-1)]^2} = \dfrac{1}{4} & \\
                  \therefore\ \text{Equation of tangent is } y - \dfrac{1}{2} & = \dfrac{1}{4}(x + 1)                  & \\
                  4y - 2                                                      & = x+1                                  & \\
                  x - 4y + 3                                                  & = 0
            \end{flalign*}
      \end{multicols}
      \vfill\null

      \newpage
      \item Find the equations of the tangent and normal to the curve $y = 1 - 2x^2$ where
            $x = -2$. \sol{}
            \begin{flalign*}
                  y              & = 1 - 2x^2 & \\
                  \dfrac{dy}{dx} & = -4x
            \end{flalign*}
            At $x = -2$, $y = 1 - 2(-2)^2 = -7$
            \begin{flalign*}
                  \text{Gradient of tangent } \dfrac{dy}{dx} & = -4(-2) = 8    & \\
                  \text{Gradient of normal }                 & = -\dfrac{1}{8}
            \end{flalign*}
            \begin{flalign*}
                  \therefore\ \text{Equation of tangent is } y + 7 & = 8(x + 2)             & \\
                  y                                                & = 8x + 9               & \\
                  \text{Equation of normal is } y + 7              & = -\dfrac{1}{8}(x + 2) & \\
                  8y + 56                                          & = -x - 2               & \\
                  x + 8y + 58                                      & = 0
            \end{flalign*}

      \item Find the equation of the tangent to the curve $y = (x+1)(x-1)(x-3)$ where the
            curve intersects with the $x$-axis. \sol{}
            \begin{flalign*}
                  y              & = (x+1)(x-1)(x-3)    & \\
                                 & = (x^2 - 1)(x-3)     & \\
                                 & = x^3 - 3x^2 - x + 3 & \\
                  \dfrac{dy}{dx} & = 3x^2 - 6x - 1
            \end{flalign*}
            At $y = 0$, $x = -1, 1, 3$.

            When $x = -1$,
            \begin{flalign*}
                  \text{Gradient of tangent } \dfrac{dy}{dx}   & = 3(-1)^2 - 6(-1) - 1 = 8 & \\
                  \therefore\ \text{Equation of tangent is } y & = 8(x + 1)                & \\
                  y                                            & = 8x + 8
            \end{flalign*}
            When $x = 1$,
            \begin{flalign*}
                  \text{Gradient of tangent } \dfrac{dy}{dx}   & = 3(1)^2 - 6(1) - 1 = -4 & \\
                  \therefore\ \text{Equation of tangent is } y & = -4(x - 1)              & \\
                  y                                            & = -4x + 4
            \end{flalign*}
            When $x = 3$,
            \begin{flalign*}
                  \text{Gradient of tangent } \dfrac{dy}{dx}   & = 3(3)^2 - 6(3) - 1 = 8 & \\
                  \therefore\ \text{Equation of tangent is } y & = 8(x - 3)              & \\
                  y                                            & = 8x - 24
            \end{flalign*}

      \item Find the equation of the tangent to the curve $y = 4x^3 - 27x + 7$ that is
            parallel to the $x$-axis. \sol{}
            \begin{flalign*}
                  y              & = 4x^3 - 27x + 7 & \\
                  \dfrac{dy}{dx} & = 12x^2 - 27
            \end{flalign*}
            The tangent is parallel to the $x$-axis when $\dfrac{dy}{dx} = 0$.
            \begin{flalign*}
                  12x^2 - 27 & = 0               & \\
                  4x^2       & = 9               & \\
                  x          & = \pm\dfrac{3}{2}
            \end{flalign*}
            When $x = \dfrac{3}{2}$, $y = 4\left(\dfrac{3}{2}\right)^3 - 27\left(\dfrac{3}{2}\right) + 7 = -20$
            \begin{flalign*}
                  \therefore\ \text{Equation of tangent is } y + 20 & = 0(x - \dfrac{3}{2}) & \\
                  y                                                 & = -20
            \end{flalign*}

            When $x = -\dfrac{3}{2}$, $y = 4\left(-\dfrac{3}{2}\right)^3 -
                  27\left(-\dfrac{3}{2}\right) + 7 = 34$
            \begin{flalign*}
                  \therefore\ \text{Equation of tangent is } y - 34 & = 0(x + \dfrac{3}{2}) & \\
                  y                                                 & = 34
            \end{flalign*}

      \item Find the equation of the tangent to the curve $y = 11x - 3x^2$ that is parallel
            to the line $x + y - 2 = 0$. \sol{}
            \begin{flalign*}
                  x + y - 2 & = 0      & \\
                  y         & = -x + 2
            \end{flalign*}
            The gradient of the line $x + y - 2 = 0$ is $-1$.
            \begin{flalign*}
                  y              & = 11x - 3x^2 & \\
                  \dfrac{dy}{dx} & = 11 - 6x
            \end{flalign*}
            The tangent is parallel to the line $x + y - 2 = 0$ when $\dfrac{dy}{dx} = -1$.
            \begin{flalign*}
                  11 - 6x & = -1 & \\
                  6x      & = 12 & \\
                  x       & = 2
            \end{flalign*}
            When $x = 2$, $y = 11(2) - 3(2)^2 = 10$
            \begin{flalign*}
                  \therefore\ \text{Equation of tangent is } y - 10 & = -1(x - 2) & \\
                  y                                                 & = -x + 12
            \end{flalign*}
            \begin{multicols}{2}
                  \item Find the equations of the tangent and normal to the curve $y = \ln{(2x - 1)}$
                  where $x=1$. \sol{}
                  \begin{flalign*}
                        y              & = \ln{(2x - 1)}     & \\
                        \dfrac{dy}{dx} & = \dfrac{2}{2x - 1}
                  \end{flalign*}
                  At $x = 1$, $y = \ln{(2(1) - 1)} = \ln{1} = 0$
                  \begin{flalign*}
                        \text{Gradient of tangent } \dfrac{dy}{dx} & = \dfrac{2}{2(1) - 1} = 2 & \\
                        \text{Gradient of normal }                 & = -\dfrac{1}{2}
                  \end{flalign*}
                  \begin{flalign*}
                        \therefore\ \text{Equation of tangent is } y - 0 & = 2(x - 1)             & \\
                        y                                                & = 2x - 2               & \\
                        \text{Equation of normal is } y - 0              & = -\dfrac{1}{2}(x - 1) & \\
                        2y                                               & = -x + 1               & \\
                        x + 2y                                           & = 1
                  \end{flalign*}
                  \item If the straight line $y = 8x + k$ is the tangent to the curve $y = x^2 + 4x -
                        3$, find the value of $k$. \sol{}

                  The gradient of the tangent line is $8$.
                  \begin{flalign*}
                        y              & = x^2 + 4x - 3 & \\
                        \dfrac{dy}{dx} & = 2x + 4       & \\
                        8              & = 2x + 4       & \\
                        x              & = 2
                  \end{flalign*}
                  When $x = 2$, $y = 2^2 + 4(2) - 3 = 9$

                  Substituting $x = 2$ and $y = 9$ into $y = 8x + k$,
                  \begin{flalign*}
                        9 & = 8(2) + k & \\
                        k & = -7
                  \end{flalign*}
            \end{multicols}

            \begin{multicols}{2}
                  \item Given that the gradient of tangent to the curve $y = ax + bx^2$ at point $(1,
                        0)$ is $\dfrac{1}{2}$, find the value of $a$ and $b$. \sol{}
                  \begin{flalign*}
                        y              & = ax + bx^2 & \\
                        \dfrac{dy}{dx} & = a + 2bx
                  \end{flalign*}
                  At point $(1, 0)$,
                  \begin{flalign*}
                        a(1) + b(1)^2                              & = 0                         & \\
                        a + b                                      & = 0\ \cdots\ (1)            & \\
                        \text{Gradient of tangent } \dfrac{dy}{dx} & = a + 2b(1) = \dfrac{1}{2}  & \\
                        a + 2b                                     & = \dfrac{1}{2}\ \cdots\ (2)
                  \end{flalign*}
                  Solving $(1)$ and $(2)$, $b = \dfrac{1}{2}$ and $a = -\dfrac{1}{2}$.
                  \vfill\null

                  \item If $x + y + 2 = 0$ is the equation of tangent to the curve $y = ax^2 + bx$
                  where $x = 1$, find the value of $a$ and $b$. \sol{}
                  \begin{flalign*}
                        x + y + 2 & = 0      & \\
                        y         & = -x - 2
                  \end{flalign*}
                  The gradient of the tangent line is $-1$.
                  \begin{flalign*}
                        y              & = ax^2 + bx & \\
                        \dfrac{dy}{dx} & = 2ax + b
                  \end{flalign*}
                  At $x = 1$, $y = -1 - 2 = -3$
                  \begin{flalign*}
                        -3                                         & = a(1)^2 + b(1)   & \\
                        a + b                                      & = -3\ \cdots\ (1) & \\
                        \text{Gradient of tangent } \dfrac{dy}{dx} & = 2a(1) + b = -1  & \\
                        2a + b                                     & = -1\ \cdots\ (2)
                  \end{flalign*}
                  Solving $(1)$ and $(2)$, $a = 2$ and $b = -5$.
            \end{multicols}

            \newpage
            \begin{multicols}{2}
                  \item Given that the gradient of tangent to the curve $y = x^3 - 6x^2 + 10x - 5$ at
                  point $P$ is $-2$, find the coordinates of $P$. \sol{}
                  \begin{flalign*}
                        y              & = x^3 - 6x^2 + 10x - 5 & \\
                        \dfrac{dy}{dx} & = 3x^2 - 12x + 10
                  \end{flalign*}
                  At point $P$, $\dfrac{dy}{dx} = -2$
                  \begin{flalign*}
                        -2              & = 3x^2 - 12x + 10 & \\
                        3x^2 - 12x + 12 & = 0               & \\
                        x^2 - 4x + 4    & = 0               & \\
                        (x - 2)^2       & = 0               & \\
                        x               & = 2
                  \end{flalign*}
                  When $x = 2$, $y = 2^3 - 6(2)^2 + 10(2) - 5 = -1$

                  $\therefore$ Coordinates of point $P$ is $(2, -1)$.
                  \vfill\null

                  \item Prove that the tangent lines to the curve $y = x^2 - 3x + 1$ and the curve
                  $x(y+3) = 4$ at point $(2, -1)$ are perpendicular to each other. \prooff{}
                  \begin{flalign*}
                        y              & = x^2 - 3x + 1 & \\
                        \dfrac{dy}{dx} & = 2x - 3
                  \end{flalign*}
                  At point $(2, -1)$,
                  \begin{flalign*}
                        \text{Gradient of tangent } \dfrac{dy}{dx} & = 2(2) - 3 = 1
                  \end{flalign*}
                  \begin{flalign*}
                        x(y+3)         & = 4                & \\
                        y              & = \dfrac{4}{x} - 3 & \\
                        \dfrac{dy}{dx} & = -\dfrac{4}{x^2}
                  \end{flalign*}
                  At point $(2, -1)$,
                  \begin{flalign*}
                        \text{Gradient of tangent } \dfrac{dy}{dx} & = -\dfrac{4}{(2)^2} = -1
                  \end{flalign*}
                  Since the product of the gradients of the two lines is $1 \times -1 = -1$, the two lines are perpendicular to each other. \qed
            \end{multicols}

            \begin{multicols}{2}
                  \item Find the equations of the tangent and normal to the curve $x^2 - xy + y^2 = 7$
                  at point $(-2, -3)$. \sol{}
                  \begin{flalign*}
                        x^2 - xy + y^2                              & = 7                      & \\
                        2x - y - x\dfrac{dy}{dx} + 2y\dfrac{dy}{dx} & = 0                      & \\
                        (2y - x) \dfrac{dy}{dx}                     & = y - 2x                 & \\
                        \dfrac{dy}{dx}                              & = \dfrac{y - 2x}{2y - x}
                  \end{flalign*}
                  At point $(-2, -3)$,
                  \begin{flalign*}
                        \text{Gradient of tangent } \dfrac{dy}{dx} & = \dfrac{-3 - 2(-2)}{2(-3) - (-2)} = -\dfrac{1}{4} & \\
                        \text{Gradient of normal }                 & = 4
                  \end{flalign*}
                  \vspace{-1cm}
                  \begin{flalign*}
                        \therefore\ \text{Equation of tangent is } y + 3 & = -\dfrac{1}{4}(x + 2) & \\
                        4y + 12                                          & = -x - 2               & \\
                        x + 4y + 14                                      & = 0                    & \\
                        \text{Equation of normal is } y + 3              & = 4(x + 2)             & \\
                        y                                                & = 4x + 5
                  \end{flalign*}

                  \item Find the equation of tangent to the curve $y^2 + y = 2\sin x$ at point $(0,
                        -1)$. \sol{}
                  \begin{flalign*}
                        y^2 + y = 2\sin x                           & \\
                        2y\dfrac{dy}{dx} + \dfrac{dy}{dx} = 2\cos x & \\
                        (2y + 1) \dfrac{dy}{dx} = 2\cos x           & \\
                        \dfrac{dy}{dx} = \dfrac{2\cos x}{2y + 1}
                  \end{flalign*}
                  At point $(0, -1)$,
                  \begin{flalign*}
                        \text{Gradient of tangent } \dfrac{dy}{dx}       & = \dfrac{2\cos 0}{2(-1) + 1} = -2 & \\
                        \therefore\ \text{Equation of tangent is } y + 1 & = -2(x - 0)                       & \\
                        y                                                & = -2x - 1
                  \end{flalign*}
            \end{multicols}
\end{enumerate}