\subsection{Exercise 27.3a}
\noindent \hspace{1.2em}\textit{Find the following indefinite integral:}
\begin{enumerate}
    \begin{multicols}{2}
        \item $\displaystyle\int(2x+1)^{3} dx$
        \sol{}

        Let $u = 2x + 1$, $du = 2dx$.
        \begin{flalign*}
            I & = \dfrac{1}{2}\int u^{3}du              & \\
              & = \dfrac{1}{2}\cdot\dfrac{u^{4}}{4} + C & \\
              & = \dfrac{1}{8}(2x + 1)^{4} + C
        \end{flalign*}

        \item $\displaystyle\int(3x+2)^{5} dx$
        \sol{}

        Let $u = 3x + 2$, $du = 3dx$.
        \begin{flalign*}
            I & = \dfrac{1}{3}\int u^{5}du              & \\
              & = \dfrac{1}{3}\cdot\dfrac{u^{6}}{6} + C & \\
              & = \dfrac{1}{18}(3x + 2)^{6} + C
        \end{flalign*}
    \end{multicols}

    \begin{multicols}{2}
        \item $\displaystyle\int(3-x)^{6} dx$
        \sol{}

        Let $u = 3 - x$, $du = -dx$.
        \begin{flalign*}
            I & = -\int u^{6}du                                       & \\
              & = -\dfrac{u^{7}}{7} + C = -\dfrac{(3 - x)^{7}}{7} + C
        \end{flalign*}

        \item $\displaystyle\int(2x-1)^{-3} dx$
        \sol{}

        Let $u = 2x - 1$, $du = 2dx$.
        \begin{flalign*}
            I & = \dfrac{1}{2}\int u^{-3}du                                               & \\
              & = \dfrac{1}{2}\cdot\dfrac{u^{-2}}{-2} + C = -\dfrac{1}{4(2x - 1)^{2}} + C
        \end{flalign*}
    \end{multicols}

    \begin{multicols}{2}
        \item $\displaystyle\int4{\sqrt{2x-1}} dx$
        \sol{}

        Let $u = 2x - 1$, $du = 2dx$.
        \begin{flalign*}
            I & = 2\int{\sqrt{u}}du                      & \\
              & = 2\cdot\dfrac{2}{3}u^{\frac{3}{2}} + C  & \\
              & = \dfrac{4}{3}(2x - 1)^{\frac{3}{2}} + C
        \end{flalign*}

        \item $\displaystyle\int2(3x+1)^{2} dx$
        \sol{}

        Let $u = 3x + 1$, $du = 3dx$.
        \begin{flalign*}
            I & = \dfrac{2}{3}\int u^{2}du              & \\
              & = \dfrac{2}{3}\cdot\dfrac{u^{3}}{3} + C & \\
              & = \dfrac{2}{9}(3x + 1)^{3} + C
        \end{flalign*}
    \end{multicols}

    \begin{multicols}{2}
        \item $\displaystyle\int\dfrac{dx}{(2x+5)^{8}}$
        \sol{}

        Let $u = 2x + 5$, $du = 2dx$.
        \begin{flalign*}
            I & = \dfrac{1}{2}\int u^{-8}du               & \\
              & = \dfrac{1}{2}\cdot\dfrac{u^{-7}}{-7} + C & \\
              & = -\dfrac{1}{14(2x + 5)^{7}} + C
        \end{flalign*}

        \item $\displaystyle\int\dfrac{2}{(3-2x)^{2}} dx$
        \sol{}

        Let $u = 3 - 2x$, $du = -2dx$.
        \begin{flalign*}
            I & = -\int\dfrac{1}{u^{2}}du & \\
              & = \dfrac{1}{u} + C        & \\
              & = \dfrac{1}{3 - 2x} + C
        \end{flalign*}
    \end{multicols}

    \begin{multicols}{2}
        \item $\displaystyle\int x{\sqrt{x^{2}+1}} dx$
        \sol{}

        Let $u = x^2 + 1$, $du = 2xdx$.
        \begin{flalign*}
            I & = \dfrac{1}{2}\int{\sqrt{u}}du                     & \\
              & = \dfrac{1}{2}\cdot\dfrac{2}{3}u^{\frac{3}{2}} + C & \\
              & = \dfrac{1}{3}(x^2 + 1)^{\frac{3}{2}} + C
        \end{flalign*}

        \item $\displaystyle\int 3x^{2}\left(x^{3}+4\right)^{3} dx$
        \sol{}

        Let $u = x^3 + 4$, $du = 3x^2dx$.
        \begin{flalign*}
            I & = \int u^{3}du                  & \\
              & = \dfrac{u^{4}}{4} + C          & \\
              & = \dfrac{1}{4}(x^3 + 4)^{4} + C
        \end{flalign*}
    \end{multicols}

    \begin{multicols}{2}
        \item $\displaystyle\int15x^{2}\left(x^{3}-1\right)^{4} dx$
        \sol{}

        Let $u = x^3 - 1$, $du = 3x^2dx$.
        \begin{flalign*}
            I \int15x^{2}\le & = \int 5u^{4}du         & \\
                             & = \dfrac{5u^{5}}{5} + C & \\
                             & = u^{5} + C             & \\
                             & = (x^3 - 1)^{5} + C
        \end{flalign*}

        \item $\displaystyle\int\left(2x+1\right)\!\left(x^{2}+x\!+\!2\right)^{5} dx$
        \sol{}

        Let $u = x^2 + x + 2$, $du = (2x + 1)dx$.
        \begin{flalign*}
            I & = \int u^{5}du                      & \\
              & = \dfrac{u^{6}}{6} + C              & \\
              & = \dfrac{1}{6}(x^2 + x + 2)^{6} + C
        \end{flalign*}
    \end{multicols}

    \newpage
    \begin{multicols}{2}
        \item $\displaystyle\int\left(x^{2}-2x\right)\left(x^{3}-3x^{2}+1\right)^{4} dx$
        \sol{}

        Let $u = x^3 - 3x^2 + 1$, $du = (3x^2 - 6x)dx$.
        \begin{flalign*}
            I & = \int u^{4}du                         & \\
              & = \dfrac{u^{5}}{5} + C                 & \\
              & = \dfrac{1}{5}(x^3 - 3x^2 + 1)^{5} + C
        \end{flalign*}

        \item $\displaystyle\int\dfrac{x+1}{{{x}^{2}}+2x+3} dx$
        \sol{}

        Let $u = x^2 + 2x + 3$, $du = (2x + 2)dx = 2(x + 1)dx$.
        \begin{flalign*}
            I & = \dfrac{1}{2}\int\dfrac{1}{u}du    & \\
              & = \dfrac{1}{2}\ln|u| + C            & \\
              & = \dfrac{1}{2}\ln|x^2 + 2x + 3| + C
        \end{flalign*}

    \end{multicols}
    \begin{multicols}{2}
        \item $\displaystyle\int x^{2}\cos\left(x^{3}+2\right) dx$
        \sol{}

        Let $u = x^3 + 2$, $du = 3x^2dx$.
        \begin{flalign*}
            I & = \dfrac{1}{3}\int\cos udu      & \\
              & = \dfrac{1}{3}\sin u + C        & \\
              & = \dfrac{1}{3}\sin(x^3 + 2) + C
        \end{flalign*}

        \item $\displaystyle\int\sin{\dfrac{x}{2}} dx$
        \sol{}

        Let $u = \dfrac{x}{2}$, $du = \dfrac{1}{2}dx$.
        \begin{flalign*}
            I & = 2\int\sin udu            & \\
              & = -2\cos u + C             & \\
              & = -2\cos{\dfrac{x}{2}} + C
        \end{flalign*}

    \end{multicols}
    \begin{multicols}{2}
        \item $\displaystyle\int\dfrac{\ln^2 x}{x} dx$
        \sol{}

        Let $u = \ln x$, $du = \dfrac{1}{x}dx$.
        \begin{flalign*}
            I & = \int u^2du              & \\
              & = \dfrac{u^3}{3} + C      & \\
              & = \dfrac{1}{3}\ln^3 x + C
        \end{flalign*}

        \item $\displaystyle\int e^{1 - 2x} dx$
        \sol{}

        Let $u = 1 - 2x$, $du = -2dx$.
        \begin{flalign*}
            I & = -\dfrac{1}{2}\int e^udu     & \\
              & = -\dfrac{1}{2}e^u + C        & \\
              & = -\dfrac{1}{2}e^{1 - 2x} + C
        \end{flalign*}

    \end{multicols}
    \begin{multicols}{2}
        \item $\displaystyle\int\left(e^{x}+e^{-x}\right) dx$
        \sol{}

        Let $u = -x$, $du = -dx$.
        \begin{flalign*}
            I & = \int e^x dx - \int e^u du & \\
              & = e^x - e^u + C             & \\
              & = e^x - e^{-x} + C
        \end{flalign*}

        \item $\displaystyle\int x e^{x^2} dx$
        \sol{}

        Let $u = x^2$, $du = 2xdx$.
        \begin{flalign*}
            I & = \dfrac{1}{2}\int e^u du & \\
              & = \dfrac{1}{2}e^u + C     & \\
              & = \dfrac{1}{2}e^{x^2} + C
        \end{flalign*}
    \end{multicols}

\end{enumerate}