\subsection{Exercise 27.5}

\begin{enumerate}
    \item Given that $\dfrac{dy}{dx} = 4x^3 - 6x^2 + 3$, and when $x = 2$, $y = 7$.
          Express $y$ in terms of $x$. \sol{}
          \begin{flalign*}
              \dfrac{dy}{dx} & = 4x^3 - 6x^2 + 3         & \\
              dy             & = (4x^3 - 6x^2 + 3)dx     & \\
              \int dy        & = \int(4x^3 - 6x^2 + 3)dx & \\
              y              & = x^4 - 2x^3 + 3x + C
          \end{flalign*}
          When $x = 2$, $y = 7$.
          \begin{flalign*}
              7 & = 16 - 16 + 6 + C & \\
              C & = 1
          \end{flalign*}
          $\therefore$ $y = x^4 - 2x^3 + 3x + 1$.
          \newpage
    \item The gradient of the tangent line of a point on a curve is $\dfrac{dy}{dx} = x^2
              + 2x - 4$, and the curve passes through point $(3, 3)$. Find the equation of
          the curve. \sol{}
          \begin{flalign*}
              \dfrac{dy}{dx} & = x^2 + 2x - 4                   & \\
              dy             & = (x^2 + 2x - 4)dx               & \\
              \int dy        & = \int(x^2 + 2x - 4)dx           & \\
              y              & = \dfrac{1}{3}x^3 + x^2 - 4x + C
          \end{flalign*}
          When $x = 3$, $y = 3$.
          \begin{flalign*}
              3 & = 9 + 9 - 12 + C & \\
              C & = -3
          \end{flalign*}
          $\therefore$ The equation of the curve is $y = \dfrac{1}{3}x^3 + x^2 - 4x - 3$.

    \item The gradient of a curve at the point $(1, -1)$ is $-4$, and $\dfrac{dy}{dx} =
              \sqrt{x} + k$. Find
          \begin{enumerate}
              \item The value of $k$. \sol{}

                    When $x = 1$, $\dfrac{dy}{dx} = -4$
                    \begin{flalign*}
                        -4 & = \sqrt{1} + k & \\
                        k  & = -5
                    \end{flalign*}

              \item The equation of the curve. \sol{}
                    \begin{flalign*}
                        \dfrac{dy}{dx} & = \sqrt{x} - 5                         & \\
                        dy             & = (\sqrt{x} - 5)dx                     & \\
                        \int dy        & = \int(\sqrt{x} - 5)dx                 & \\
                        y              & = \dfrac{2}{3}x^{\frac{3}{2}} - 5x + C
                    \end{flalign*}
                    When $x = 1$, $y = -1$.
                    \begin{flalign*}
                        -1 & = \dfrac{2}{3} - 5 + C & \\
                        C  & = \dfrac{10}{3}
                    \end{flalign*}
                    $\therefore$ The equation of the curve is $y = \dfrac{2}{3}x^{\frac{3}{2}} - 5x + \dfrac{10}{3}$.

          \end{enumerate}
\end{enumerate}