\subsection{Exercise 27.4}

\noindent \hspace{1.2em}\textit{Find the following indefinite integral:}
\begin{enumerate}
    \begin{multicols}{2}
        \item $\displaystyle\int\dfrac{1}{x(x+1)} dx$
        \sol{}

        Let $\dfrac{1}{x(x+1)} = \dfrac{A}{x} + \dfrac{B}{x+1}$.
        \begin{flalign*}
            \dfrac{1}{x(x+1)} & = \dfrac{A}{x} + \dfrac{B}{x+1} & \\
            1                 & = Ax + A + Bx                   & \\
                              & = (A + B)x + A
        \end{flalign*}
        \vspace{-2em}
        \begin{flalign*}
            \begin{cases}
                A + B = 0 \\
                A = 1
            \end{cases}
            \Rightarrow
            \begin{cases}
                A = 1 \\
                B = -1
            \end{cases}
        \end{flalign*}
        \vspace{-1em}
        \begin{flalign*}
            I & = \int\left(\dfrac{1}{x} - \dfrac{1}{x+1}\right) dx & \\
              & = \ln|x| - \ln|x+1| + C
        \end{flalign*}

        \item $\displaystyle\int\dfrac{x}{(x+1)(x-3)} dx$
        \sol{}

        Let $\dfrac{x}{(x+1)(x-3)} = \dfrac{A}{x+1} + \dfrac{B}{x-3}$.
        \begin{flalign*}
            \dfrac{x}{(x+1)(x-3)} & = \dfrac{A}{x+1} + \dfrac{B}{x-3} & \\
            x                     & = Ax - 3A + Bx + B                & \\
                                  & = (A + B)x + (-3A + B)
        \end{flalign*}
        \vspace{-2em}
        \begin{flalign*}
            \begin{cases}
                A + B = 1 \\
                -3A + B = 0
            \end{cases}
            \Rightarrow
            \begin{cases}
                A = \dfrac{1}{4} \\
                B = \dfrac{3}{4}
            \end{cases}
        \end{flalign*}
        \vspace{-1em}
        \begin{flalign*}
            I & = \int\left(\dfrac{1}{4}\cdot\dfrac{1}{x+1} + \dfrac{3}{4}\cdot\dfrac{1}{x-3}\right) dx & \\
              & = \dfrac{1}{4}\ln|x+1| + \dfrac{3}{4}\ln|x-3| + C
        \end{flalign*}
    \end{multicols}

    \begin{multicols}{2}
        \item $\displaystyle\int\dfrac{4x-13}{2x^2+x-6} dx$
        \sol{}

        Let $\dfrac{4x-13}{2x^2+x-6} = \dfrac{A}{2x-3} + \dfrac{B}{x+2}$.
        \begin{flalign*}
            \dfrac{4x-13}{2x^2+x-6} & = \dfrac{A}{2x-3} + \dfrac{B}{x+2} & \\
            4x - 13                 & = Ax + 2A + 2Bx - 3B               & \\
                                    & = (A + 2B)x + (2A - 3B)
        \end{flalign*}
        \vspace{-2em}
        \begin{flalign*}
            \begin{cases}
                A + 2B = 4 \\
                2A - 3B = -13
            \end{cases}
            \Rightarrow
            \begin{cases}
                A = -2 \\
                B = 3
            \end{cases}
        \end{flalign*}
        \vspace{-1em}
        \begin{flalign*}
            I & = \int\left(\dfrac{-2}{2x-3} + \dfrac{3}{x+2}\right) dx & \\
              & = 3\ln|x+2| -\ln|2x-3|+ C
        \end{flalign*}

        \item $\displaystyle\int\dfrac{5x-1}{1-x^{2}} dx$
        \sol{}

        Let $\dfrac{5x-1}{1-x^{2}} = \dfrac{A}{1-x} + \dfrac{B}{1+x}$.
        \begin{flalign*}
            \dfrac{5x-1}{1-x^{2}} & = \dfrac{A}{1-x} + \dfrac{B}{1+x} & \\
            5x - 1                & = A + Ax + B - Bx                 & \\
                                  & = (A - B)x + (A + B)
        \end{flalign*}
        \vspace{-2em}
        \begin{flalign*}
            \begin{cases}
                A - B = 5 \\
                A + B = -1
            \end{cases}
            \Rightarrow
            \begin{cases}
                A = 2 \\
                B = -3
            \end{cases}
        \end{flalign*}
        \vspace{-1em}
        \begin{flalign*}
            I & = \int\left(\dfrac{2}{1-x} - \dfrac{3}{1+x}\right) dx & \\
              & = -2\ln|1-x| - 3\ln|1+x| + C
        \end{flalign*}
    \end{multicols}

    \newpage

    \begin{multicols}{2}
        \item $\displaystyle\int\dfrac{x^{2}+5}{(x+1)(x-1)} dx$
        \sol{}
        \begin{flalign*}
            I & = \int\dfrac{x^{2}+5}{x^2 - 1}               & \\
              & = \int\left(1 + \dfrac{6}{x^2 - 1}\right) dx
        \end{flalign*}
        Let $\dfrac{6}{x^2 - 1} = \dfrac{A}{x-1} + \dfrac{B}{x+1}$.
        \begin{flalign*}
            \dfrac{6}{x^2 - 1} & = \dfrac{A}{x-1} + \dfrac{B}{x+1} & \\
            6                  & = Ax + A + Bx - B                 & \\
                               & = (A + B)x + (A - B)
        \end{flalign*}
        \vspace{-2em}
        \begin{flalign*}
            \begin{cases}
                A + B = 0 \\
                A - B = 6
            \end{cases}
            \Rightarrow
            \begin{cases}
                A = 3 \\
                B = -3
            \end{cases}
        \end{flalign*}
        \vspace{-1em}
        \begin{flalign*}
            I & = \int\left(1 + \dfrac{3}{x-1} - \dfrac{3}{x+1}\right) dx & \\
              & = x + 3\ln|x-1| - 3\ln|x+1| + C
        \end{flalign*}

        \item $\displaystyle\int\dfrac{x^{3}+2}{x^{2}-1} dx$
        \sol{}
        \begin{flalign*}
            I & = \int\dfrac{x^{3}+2}{x^{2}-1} dx                 & \\
              & = \int \left(x + \dfrac{x + 2}{x^{2}-1}\right) dx
        \end{flalign*}
        Let $\dfrac{x + 2}{x^{2}-1} = \dfrac{A}{x-1} + \dfrac{B}{x+1}$.
        \begin{flalign*}
            \dfrac{x + 2}{x^{2}-1} & = \dfrac{A}{x-1} + \dfrac{B}{x+1} & \\
            x + 2                  & = Ax + A + Bx - B                 & \\
                                   & = (A + B)x + (A - B)
        \end{flalign*}
        \vspace{-2em}
        \begin{flalign*}
            \begin{cases}
                A + B = 1 \\
                A - B = 2
            \end{cases}
            \Rightarrow
            \begin{cases}
                A = \dfrac{3}{2} \\
                B = -\dfrac{1}{2}
            \end{cases}
        \end{flalign*}
        \vspace{-1em}
        \begin{flalign*}
            I & = \int\left(x + \dfrac{3}{2}\cdot\dfrac{1}{x-1} - \dfrac{1}{2}\cdot\dfrac{1}{x+1}\right) dx & \\
              & = \dfrac{1}{2}x^2 + \dfrac{3}{2}\ln|x-1| - \dfrac{1}{2}\ln|x+1| + C
        \end{flalign*}
    \end{multicols}

    \begin{multicols}{2}
        \item $\displaystyle\int\dfrac{2x-1}{x^{2}+2x+1} dx$
        \sol{}
        \begin{flalign*}
            I & = \int\dfrac{2x-1}{(x+1)^2} dx
        \end{flalign*}
        Let $u = x + 1$, $du = dx$, $x = u - 1$.
        \begin{flalign*}
            I & = \int\dfrac{2u - 3}{u^2} du     & \\
              & = \int(2u^{-1} - 3u^{-2}) du     & \\
              & = 2\ln|u| + \dfrac{3}{u} + C     & \\
              & = 2\ln|x+1| + \dfrac{3}{x+1} + C
        \end{flalign*}

        \item $\displaystyle\int\dfrac{4x-3}{(2x+1)^{2}} dx$
        \sol{}

        Let $u = 2x + 1$, $du = 2dx$, $x = \dfrac{u - 1}{2}$.
        \begin{flalign*}
            I & = \dfrac{1}{2}\int\dfrac{2u - 5}{u^2}du  & \\
              & = \dfrac{1}{2}\int(2u^{-1} - 5u^{-2})du  & \\
              & = \ln|u| + \dfrac{5}{2u} + C             & \\
              & = \ln|2x + 1| + \dfrac{5}{2(2x + 1)} + C
        \end{flalign*}
    \end{multicols}
\end{enumerate}