\section{Revision Exercise 27}

Find the following indefinite integral (Question 1 to 34):
\begin{enumerate}
    \begin{multicols}{2}
        \item $\displaystyle\int 2x^{\frac{1}{5}}dx$
        \sol{}
        \begin{flalign*}
            I & = 2 \cdot \dfrac{5}{6}x^{\frac{6}{5}} + C & \\
              & = \dfrac{5}{3}x^{\frac{6}{5}} + C
        \end{flalign*}
        \vfill{}\null{}
        \item $\displaystyle\int{(2x-1)}^3dx$
        \sol{}
        \begin{flalign*}
            I & = \dfrac{1}{2}\int{(2x-1)}^3d(2x-1)             & \\
              & = \dfrac{1}{2} \cdot \dfrac{1}{4}{(2x-1)}^4 + C & \\
              & = \dfrac{1}{8}{(2x-1)}^4 + C
        \end{flalign*}
    \end{multicols}

    \begin{multicols}{2}
        \item $\displaystyle\int{(x+4)}^{100}dx$
        \sol{}
        \begin{flalign*}
            I & = \int{(x+4)}^{100}d(x+4)         & \\
              & = \dfrac{1}{101}{(x+4)}^{101} + C
        \end{flalign*}
        \item $\displaystyle\int{\left(\dfrac{5}{x^2}+2x^{\frac{1}{2}}+3\right)}dx$
        \sol{}
        \begin{flalign*}
            I & =5\int{x^{-2}} + 2\int{x^{\frac{1}{2}}} + 3\int dx     & \\
              & = -\dfrac{5}{x} + \dfrac{4}{3}x^{\frac{3}{2}} + 3x + C
        \end{flalign*}
    \end{multicols}

    \begin{multicols}{2}
        \item $\displaystyle\int{\left(3x^2 + \dfrac{1}{x^2} - \sin x\right)}dx$
        \sol{}
        \begin{flalign*}
            I & = 3\int x^2 + \int x^{-2} - \int \sin x dx & \\
              & = x^3 - x^{-1} + \cos x + C                & \\
              & = x^3 + \dfrac{1}{x} + \cos x + C
        \end{flalign*}
        \item $\displaystyle\int{\left(4\cos x + \dfrac{1}{x} + x^3\right)}dx$
        \sol{}
        \begin{flalign*}
            I & = 4\int \cos x + \int x^{-1} + \int x^3 dx          & \\
              & = 4\sin x + \ln \vert x \vert + \dfrac{1}{4}x^4 + C
        \end{flalign*}
    \end{multicols}

    \begin{multicols}{2}
        \item $\displaystyle\int\dfrac{3x^3 - 2x^2 + x^{-1}}{x^2}dx$
        \sol{}
        \begin{flalign*}
            I & = \int(3x - 2 + x^{-3})dx                       & \\
              & = \dfrac{3}{2}x^2 - 2x - \dfrac{1}{2}x^{-2} + C
        \end{flalign*}
        \item $\displaystyle\int(2x-1)(x+2)dx$
        \sol{}
        \begin{flalign*}
            I & = \int(2x^2 + 3x - 2)dx                      & \\
              & = \dfrac{2}{3}x^3 + \dfrac{3}{2}x^2 - 2x + C
        \end{flalign*}
    \end{multicols}

    \begin{multicols}{2}
        \item $\displaystyle\int{\left(x-\dfrac{1}{x^2}\right)}^2dx$
        \sol{}
        \begin{flalign*}
            I & = \int(x^2 - 2x^{-1} + x^{-4})dx                                & \\
              & = \dfrac{1}{3}x^3 - 2\ln \vert x \vert - \dfrac{1}{3}x^{-3} + C
        \end{flalign*}
        \item $\displaystyle\int{\left(x + \dfrac{1}{x}\right)}^3dx$
        \sol{}
        \begin{flalign*}
            I & = \int(x^3 + 3x + 3x^{-1} + x^{-3})dx                                             & \\
              & = \dfrac{1}{4}x^4 + \dfrac{3}{2}x^2 + 3\ln \vert x \vert - \dfrac{1}{2}x^{-2} + C
        \end{flalign*}
    \end{multicols}
    \newpage
    \begin{multicols}{2}
        \item $\displaystyle\int10^{-x}dx$
        \sol{}
        \begin{flalign*}
            I & = -\int10^{-x}d(-x)            & \\
              & = -\dfrac{10^{-x}}{\ln 10} + C & \\
              & = -\dfrac{1}{10^{x}\ln 10} + C
        \end{flalign*}
        \item $\displaystyle\int{\left(e^x - e^{-x}\right)}^2dx$
        \sol{}
        \begin{flalign*}
            I & = \int(e^{2x} - 2 + e^{-2x})dx                      & \\
              & = \dfrac{1}{2}e^{2x} - 2x - \dfrac{1}{2}e^{-2x} + C
        \end{flalign*}
    \end{multicols}

    \begin{multicols}{2}
        \item $\displaystyle\int2x{(x^2 - 1)}^4dx$
        \sol{}
        \begin{flalign*}
            I & = \int{(x^2 - 1)}^4d(x^2 - 1)   & \\
              & = \dfrac{1}{5}{(x^2 - 1)}^5 + C
        \end{flalign*}
        \item $\displaystyle\int3x^2{(x^3 + 1)}^4dx$
        \sol{}
        \begin{flalign*}
            I & = \int{(x^3 + 1)}^4d(x^3 + 1)   & \\
              & = \dfrac{1}{5}{(x^3 + 1)}^5 + C
        \end{flalign*}
    \end{multicols}

    \begin{multicols}{2}
        \item $\displaystyle\int\dfrac{x+1}{{(x^2 + 2x + 5)}^3}dx$
        \sol{}
        \begin{flalign*}
            I & = \dfrac{1}{2}\int\dfrac{1}{(x^2 + 2x + 5)^3}d(x^2 + 2x + 5) & \\
              & = -\dfrac{1}{4(x^2 + 2x + 5)^2} + C
        \end{flalign*}
        \item $\displaystyle\int\dfrac{2x}{\sqrt{x^2-4}}dx$
        \sol{}
        \begin{flalign*}
            I & = \int\dfrac{1}{\sqrt{x^2-4}}d(x^2-4) & \\
              & = 2\sqrt{x^2-4} + C
        \end{flalign*}
    \end{multicols}

    \begin{multicols}{2}
        \item $\displaystyle\int\dfrac{x-2}{\sqrt{(x-1)(x-3)}}dx$
        \sol{}
        \begin{flalign*}
            I & = \int\dfrac{x-2}{\sqrt{x^2-4x+3}}dx                    & \\
              & = \dfrac{1}{2}\int\dfrac{1}{\sqrt{x^2-4x+3}}d(x^2-4x+3) & \\
              & = \dfrac{1}{2}\cdot 2\sqrt{x^2-4x+3} + C                & \\
              & = \sqrt{x^2-4x+3} + C
        \end{flalign*}
        \vfill{}\null{}
        \columnbreak
        \item $\displaystyle\int\dfrac{7}{2x^2 + 5x - 3}dx$
        \sol{}
        \begin{flalign*}
            I = \int\dfrac{7}{(2x - 1)(x + 3)}dx &
        \end{flalign*}
        \vspace{-2em}
        \begin{flalign*}
            \text{Let } \dfrac{7}{(2x - 1)(x + 3)} & = \dfrac{A}{2x - 1} + \dfrac{B}{x + 3} & \\
            A(x + 3) + B(2x - 1)                   & = 7                                    & \\
            (A + 2B)x + (3A - B)                   & = 7
        \end{flalign*}
        Comparing coefficients,
        \begin{flalign*}
            A + 2B    & = 0  & \\
            3A - B    & = 7  & \\
            A = 2,\ B & = -1
        \end{flalign*}
        \vspace{-2em}
        \begin{flalign*}
            I & = \int\left(\dfrac{2}{2x-1} - \dfrac{1}{x + 3}\right)dx & \\
              & = \int\dfrac{2}{2x-1}dx - \int\dfrac{1}{x + 3}dx        & \\
              & = \ln|2x - 1| - \ln|x + 3| + C                          & \\
              & = \ln\left|\dfrac{2x - 1}{x + 3}\right| + C
        \end{flalign*}
    \end{multicols}

    \begin{multicols}{2}
        \item $\displaystyle\int\dfrac{8 - 7x}{2 + x - 3x^2}dx$
        \sol{}
        \begin{flalign*}
            I & = -\int\dfrac{7x + 8}{(3x + 2)(x - 1)}dx
        \end{flalign*}
        \vspace{-2em}
        \begin{flalign*}
            \text{Let } \dfrac{7x + 8}{(3x + 2)(x - 1)} & = \dfrac{A}{3x + 2} + \dfrac{B}{x - 1} & \\
            A(x - 1) + B(3x + 2)                        & = 7x + 8                               & \\
            (A + 3B)x + (-A + 2B)                       & = 7x + 8
        \end{flalign*}
        Comparing coefficients,
        \begin{flalign*}
            A + 3B     & = 7 & \\
            -A + 2B    & = 8 & \\
            A = -2,\ B & = 3
        \end{flalign*}
        \vspace{-2em}
        \begin{flalign*}
            I & = -\int\left(-\dfrac{2}{3x + 2} + \dfrac{3}{x - 1}\right)dx & \\
              & = -\int-\dfrac{2}{3x + 2}dx - \int\dfrac{3}{x - 1}dx        & \\
              & = \dfrac{2}{3}\ln|3x + 2| - 3\ln|x - 1| + C                 & \\
        \end{flalign*}
        \item $\displaystyle\int\dfrac{x+1}{(3x+2)(5x+3)}dx$
        \sol{}
        \vspace{-2em}
        \begin{flalign*}
            \text{Let } \dfrac{x+1}{(3x+2)(5x+3)} & = \dfrac{A}{3x+2} + \dfrac{B}{5x+3} & \\
            A(5x + 3) + B(3x + 2)                 & = x + 1                             & \\
            (5A + 3B)x + (3A + 2B)                & = x + 1
        \end{flalign*}
        Comparing coefficients,
        \begin{flalign*}
            5A + 3B    & = 1 & \\
            3A + 2B    & = 1 & \\
            A = -1,\ B & = 2
        \end{flalign*}
        \begin{flalign*}
            I & = \int\left(\dfrac{-1}{3x+2} + \dfrac{2}{5x+3}\right)dx  & \\
              & = -\int\dfrac{1}{3x+2}dx + \int\dfrac{2}{5x+3}dx         & \\
              & = -\dfrac{1}{3}\ln|3x + 2| + \dfrac{2}{5}\ln|5x + 3| + C & \\
        \end{flalign*}
    \end{multicols}

    \begin{multicols}{2}
        \item $\displaystyle\int\dfrac{2x^2 + 5x - 2}{2x^2 + x - 3}dx$
        \sol{}
        \begin{flalign*}
            I & = \int\left(1 + \dfrac{4x + 1}{2x^2 + x - 3}\right)dx          & \\
              & = \int\left[1 + \dfrac{(2x^2 + x - 3)'}{2x^2 + x - 3}\right]dx & \\
              & = x + \ln\vert2x^2 + x - 3\vert + C
        \end{flalign*}
        \item $\displaystyle\int{\left(\dfrac{x+1}{x-1}\right)}^2dx$
        \sol{}
        \begin{flalign*}
            I & = \int\left(1 + \dfrac{2}{x-1}\right)^2dx                    & \\
              & = \int\left[1 + \dfrac{4}{x-1} + \dfrac{4}{(x-1)^2}\right]dx & \\
              & = x + 4\ln\vert x - 1\vert - \dfrac{4}{x - 1} + C
        \end{flalign*}
    \end{multicols}

    \begin{multicols}{2}
        \item $\displaystyle\int\dfrac{{(x-1)}^3}{{(x-2)}^2}dx$
        \sol{}

        Let $u = x - 2$, $du = dx$.
        \begin{flalign*}
            I & = \int\dfrac{{(u+1)}^3}{u^2}du                                                &   & \\
              & = \int\left(\dfrac{u^3 + 3u^2 + 3u + 1}{u^2}\right)du                         &     \\
              & = \int\left(u + 3 + \dfrac{3}{u} + \dfrac{1}{u^2}\right)du                    &     \\
              & = \dfrac{u^2}{2} + 3u + 3\ln\vert u\vert - \dfrac{1}{u} + C                   &     \\
              & = \dfrac{x^2 - 4x + 4 + 6x - 12}{2} + 3\ln\vert x-2\vert - \dfrac{1}{x-2} + C &     \\
              & = \dfrac{1}{2}x^2 + x + 3\ln\vert x-2\vert - \dfrac{1}{x-2} + C
        \end{flalign*}
        \item $\displaystyle\int\dfrac{x^2}{{(x+2)}^3}dx$
        \sol{}

        Let $u = x + 2$, $du = dx$.
        \begin{flalign*}
            I & = \int\dfrac{{(u-2)}^2}{u^3}du                                      & \\
              & = \int\left(\dfrac{u^2 - 4u + 4}{u^3}\right)du                      & \\
              & = \int\left(\dfrac{1}{u} - \dfrac{4}{u^2} + \dfrac{4}{u^3}\right)du & \\
              & = \ln\vert u\vert + \dfrac{4}{u} - \dfrac{2}{u^2} + C               & \\
              & = \ln\vert x+2\vert + \dfrac{4}{x+2} - \dfrac{2}{(x+2)^2} + C
        \end{flalign*}
    \end{multicols}

    \begin{multicols}{2}
        \item $\displaystyle\int\left(3\sin2x-4e^{3x}\right)dx$
        \sol{}
        \begin{flalign*}
            I & = \dfrac{3}{2}\int\sin2xd(2x) - \int4e^{3x}dx  & \\
              & = -\dfrac{3}{2}\cos2x - \dfrac{4}{3}e^{3x} + C & \\
        \end{flalign*}
        \item $\displaystyle\int\sin(5x-6)dx$
        \sol{}
        \begin{flalign*}
            I & = \dfrac{1}{5}\int\sin(5x-6)d(5x-6) & \\
              & = -\dfrac{1}{5}\cos(5x-6) + C
        \end{flalign*}
    \end{multicols}

    \begin{multicols}{2}
        \item $\displaystyle\int\left(\cos6x+\sec^2 4x\right)dx$
        \sol{}
        \begin{flalign*}
            I & = \dfrac{1}{6}\int\cos6xd(6x) + \dfrac{1}{4}\int\sec^2 4xd(4x) & \\
              & = \dfrac{1}{6}\sin6x + \dfrac{1}{4}\tan4x + C
        \end{flalign*}
        \item $\displaystyle\int\left(\sin\dfrac{x}{2}+\cos2x-\cos\dfrac{x}{7}\right)dx$
        \sol{}
        \begin{flalign*}
            I & = 2\int\sin\dfrac{x}{2}d\left(\dfrac{x}{2}\right) + \int\cos2xd(2x) & \\
              & \ \ \ \ - 7\int\cos\dfrac{x}{7}d\left(\dfrac{x}{7}\right)           & \\
              & = -2\cos\dfrac{x}{2} + \dfrac{1}{2}\sin2x - 7\sin\dfrac{x}{7} + C
        \end{flalign*}
    \end{multicols}

    \begin{multicols}{2}
        \item $\displaystyle\int\tan^2 3xdx$
        \sol{}
        \begin{flalign*}
            I & = \int\left(\sec^2 3x - 1\right)dx         & \\
              & = \dfrac{1}{3}\int\sec^2 3xd(3x) - \int dx & \\
              & = \dfrac{1}{3}\tan3x - x + C
        \end{flalign*}
        \item $\displaystyle\int\tan x\sec^2 xdx$
        \sol{}
        \begin{flalign*}
            I & = \int\tan xd(\tan x)      & \\
              & = \dfrac{1}{2}\tan^2 x + C
        \end{flalign*}
    \end{multicols}

    \begin{multicols}{2}
        \item $\displaystyle\int\dfrac{3\sin x}{\cos2x + 1}dx$
        \sol{}
        \begin{flalign*}
            I & = \int\dfrac{3\sin x}{2\cos^2 x}dx           & \\
              & = \dfrac{3}{2}\int\dfrac{\sin x}{\cos^2 x}dx & \\
              & = \dfrac{3}{2}\int\sec x\tan xdx             & \\
              & = \dfrac{3}{2}\sec x + C
        \end{flalign*}
        \item $\displaystyle\int\dfrac{\sec^2 x}{\tan x + 2}dx$
        \sol{}
        \begin{flalign*}
            I & = \int\dfrac{1}{\tan x + 2}d(\tan x) & \\
              & = \ln\vert\tan x + 2\vert + C
        \end{flalign*}
    \end{multicols}

    \begin{multicols}{2}
        \item $\displaystyle\int\cot2x\csc^3 2xdx$
        \sol{}
        \begin{flalign*}
            I & = \int\csc 2x \cot 2x \csc^2 2xdx     & \\
              & = \dfrac{1}{2}\int\csc^2 2xd(\csc 2x) & \\
              & = -\dfrac{1}{6}\csc^3 2x + C
        \end{flalign*}
        \vfill{}\null{}
        \item $\displaystyle\int\tan^3 x\sec^3 xdx$
        \sol{}
        \begin{flalign*}
            I & = \int\tan^2 x\sec^2 x\sec x\tan xdx                  & \\
              & = \int\left(\sec^2 x - 1\right)\sec^2 x\sec x\tan xdx & \\
              & = \int\left(\sec^4 x - \sec^2 x\right)d(\sec x)       & \\
              & = \dfrac{1}{5}\sec^5 x - \dfrac{1}{3}\sec^3 x + C
        \end{flalign*}
    \end{multicols}

    \item If the function $y = \ln x - \dfrac{3}{x}$, find $\dfrac{dy}{dx}$. Hence, find
          $\displaystyle\int\dfrac{3+x}{3x^2}dx$. \sol{}
          \begin{flalign*}
              y                       & = \ln x - \dfrac{3}{x}                   & \\
              \dfrac{dy}{dx}          & = \dfrac{1}{x} + \dfrac{3}{x^2}          & \\
                                      & = \dfrac{x+3}{x^2}                       & \\
                                      &                                            \\
              \int\dfrac{3+x}{3x^2}dx & = \dfrac{1}{3}\int\dfrac{x+3}{x^2}d(x^3) & \\
                                      & = \dfrac{1}{3}\ln x - \dfrac{1}{x} + C
          \end{flalign*}

    \item If the function $y = \dfrac{1}{\sqrt{4x^2 - 1}}$, find $\dfrac{dy}{dx}$. Hence,
          find $\displaystyle\int\dfrac{x}{\sqrt{{\left(4x^2-1\right)}^3}}$. \sol{}
          \begin{flalign*}
              y                                               & = \left[\left(4x^2 - 1\right)^{-\dfrac{1}{2}}\right]'                 & \\
                                                              & = -\dfrac{1}{2}\left(4x^2 - 1\right)^{-\dfrac{3}{2}}\cdot 8x          & \\
                                                              & = -\dfrac{4x}{\sqrt{{\left(4x^2-1\right)}^3}}                         & \\
                                                              &                                                                         \\
              \int\dfrac{x}{\sqrt{{\left(4x^2-1\right)}^3}}dx & = -\dfrac{1}{4}\int-\dfrac{4x}{\sqrt{{\left(4x^2-1\right)}^3}}d(4x^2) & \\
                                                              & = -\dfrac{1}{4\sqrt{4x^2-1}} + C
          \end{flalign*}

    \item Given the function $y = \dfrac{x^2 + 3}{1-x}$, and $\dfrac{dy}{dx} =
              \dfrac{1}{2}f(x)$, find $\displaystyle\int\left[3 - x^2 - f(x)\right]dx$.
          \sol{}
          \begin{flalign*}
              \dfrac{d}{dx}\left(\dfrac{x^2 + 3}{1-x}\right) & = \dfrac{1}{2}f(x)                                                                           & \\
              f(x)                                           & = 2\left[\dfrac{d}{dx}\left(\dfrac{x^2 + 3}{1-x}\right)\right]                               & \\
                                                             &                                                                                                \\
              \int\left[3 - x^2 - f(x)\right]dx              & = \int3dx - \int x^2dx - f(x)dx                                                              & \\
                                                             & = \int3dx - \int x^2dx - \int 2\left[\dfrac{d}{dx}\left(\dfrac{x^2 + 3}{1-x}\right)\right]dx & \\
                                                             & = 3x - \dfrac{x^3}{3} - \dfrac{2(x^2 + 3)}{1-x} + C
          \end{flalign*}

          \newpage

    \item Given the function $\dfrac{d}{dx}(x\ln x) = g(x)$, find
          $\displaystyle\int\left[g(x) - 2x\right]dx$. \sol{}
          \begin{flalign*}
              \int\left[g(x) - 2x\right]dx & = \int g(x)dx - \int 2xdx                  & \\
                                           & = \int \dfrac{d}{dx}(x\ln x)dx - \int 2xdx & \\
                                           & = x\ln x - x^2 + C
          \end{flalign*}

    \item The gradient of the tangent at any point on a curve is 3 times the
          $x$-coordinate of the point, and the curve passes through $(-2, 5)$. Find the
          equation of the curve. \sol{}
          \begin{flalign*}
              \dfrac{dy}{dx} & = 3x                  & \\
              dy             & = 3xdx                & \\
              y              & = \dfrac{3}{2}x^2 + C
          \end{flalign*}
          Given that the curve passes through $(-2, 5)$,
          \begin{flalign*}
              5 & = \dfrac{3(-2)^2}{2} + C & \\
              C & = 1
          \end{flalign*}
          Therefore, the equation of the curve is $y = \dfrac{3}{2}x^2 + 1$.

    \item The gradient of the tangent at any point on a curve is $\dfrac{dy}{dx} = 3x^2 -
              8x + 1$, and the curve intersect with $x$-axis at point $(2, 0)$, find the
          other point of intersection of the curve and the $x$-axis. \sol{}
          \begin{flalign*}
              \dfrac{dy}{dx} & = 3x^2 - 8x + 1          & \\
              y              & = \int (3x^2 - 8x + 1)dx & \\
                             & = x^3 - 4x^2 + x + C
          \end{flalign*}
          Given that the curve passes through $(2, 0)$,
          \begin{flalign*}
              0 & = 2^3 - 4(2)^2 + 2 + C & \\
              C & = -6
          \end{flalign*}
          Therefore, the equation of the curve is $y = x^3 - 4x^2 + x -6$.

          When the curve intersects with the $x$-axis, $y = 0$,
          \begin{flalign*}
              x^3 - 4x^2 + x + 6 & = 0 & \\
              (x-2)(x^2-2x-3)    & = 0 & \\
              (x-2)(x-3)(x+1)    & = 0
          \end{flalign*}
          Therefore, the curve also intersects with the $x$-axis at $(-1, 0)$ and $(3, 0)$.
\end{enumerate}