\subsection{Exercise 28.2}

\begin{enumerate}
    \begin{multicols}{2}
        \item $\displaystyle\int_0^4\left(x^2-2 x\right) d x$
        \sol{}
        \begin{flalign*}
            I & = \bigg[\dfrac{1}{3}x^3 - x^2\bigg]_0^4 & \\
              & = \dfrac{64}{3} - 16                    & \\
              & = \dfrac{16}{3}
        \end{flalign*}
        \item $\displaystyle\int_1^4 \dfrac{2 x^2-3 \sqrt{x}+1}{x} d x$
        \sol{}
        \begin{flalign*}
            I & = \int_1^4 \left(2x - 3x^{-\frac{1}{2}} + x^{-1}\right) d x & \\
              & = \bigg[x^2 - 6\sqrt{x} + \ln|x|\bigg]_1^4                  & \\
              & = 16 - 12 + \ln 4 - 1 + 6 - \ln 1                           & \\
              & = 9 + \ln 4
        \end{flalign*}
    \end{multicols}

    \begin{multicols}{2}
        \item $\displaystyle\int_{-3}^3(x+3)^2 d x$
        \sol{}

        Let $u = x + 3$, $du = dx$.

        When $x = -3$, $u = 0$.

        When $x = 3$, $u = 6$.
        \begin{flalign*}
            I & = \int_0^6 u^2 d u                & \\
              & = \bigg[\dfrac{1}{3}u^3\bigg]_0^6 & \\
              & = 72
        \end{flalign*}

        \item $\displaystyle\int_{-1}^1(2+x)\left(2-x^2\right) d x$
        \sol{}
        \begin{flalign*}
            I & = \int_{-1}^1\left(4 - 2x^2 + 2x - x^3\right)dx                             & \\
              & = \bigg[4x - \dfrac{2}{3}x^3 + x^2 - \dfrac{1}{4}x^4\bigg]_{-1}^1           & \\
              & = 4 - \dfrac{2}{3} + 1 - \dfrac{1}{4} + 4 - \dfrac{2}{3} - 1 + \dfrac{1}{4} & \\
              & = \dfrac{20}{3}
        \end{flalign*}
    \end{multicols}

    \begin{multicols}{2}
        \item $\displaystyle\int_0^{\frac{\pi}{2}}(2 \sin 3 \theta-3 \cos 2 \theta) d \theta$
        \sol{}
        \begin{flalign*}
            I & = \bigg[-\dfrac{2}{3}\cos 3\theta - \dfrac{3}{2}\sin 2\theta\bigg]_0^{\frac{\pi}{2}} & \\
              & = \dfrac{2}{3} + \dfrac{3}{2} + \dfrac{2}{3}                                         & \\
              & = \dfrac{13}{6}
        \end{flalign*}
        \vfill{}\null{}
        \columnbreak{}

        \item $\displaystyle\int_0^{\frac{\pi}{3}} \tan \theta d \theta$
        \sol{}
        \begin{flalign*}
            I & = \int_0^{\frac{\pi}{3}} \dfrac{\sin \theta}{\cos \theta} d \theta &
        \end{flalign*}
        Let $u = \cos \theta$, $du = -\sin \theta d \theta$.

        When $\theta = 0$, $u = 1$.

        When $\theta = \dfrac{\pi}{3}$, $u = \dfrac{1}{2}$.
        \begin{flalign*}
            I & = -\int_1^{\frac{1}{2}} \dfrac{1}{u} d u & \\
              & = -\bigg[\ln|u|\bigg]_1^{\frac{1}{2}}    & \\
              & = -\ln\dfrac{1}{2} + \ln 1               & \\
              & = \ln 2
        \end{flalign*}
    \end{multicols}

    \newpage

    \begin{multicols}{2}
        \item $\displaystyle\int_0^1\left(e^x-1\right)^2 d x$
        \sol{}
        \begin{flalign*}
            I & = \int_0^1\left(e^{2x} - 2e^x + 1\right) d x    & \\
              & = \bigg[\dfrac{1}{2}e^{2x} - 2e^x + x\bigg]_0^1 & \\
              & = \dfrac{1}{2}e^2 - 2e + 1 - \dfrac{1}{2} + 2   & \\
              & = \dfrac{1}{2}e^2 - 2e + \dfrac{5}{2}           & \\
              & = \dfrac{e^2 - 4e + 5}{2}
        \end{flalign*}
        \vfill{}\null{}

        \item $\displaystyle\int_1^4 \dfrac{2}{4 x-1} d x$
        \sol{}

        Let $u = 4x - 1$, $du = 4dx$.

        When $x = 1$, $u = 3$.

        When $x = 4$, $u = 15$.
        \begin{flalign*}
            I & = \dfrac{1}{2}\int_3^{15} \dfrac{1}{u} d u & \\
              & = \dfrac{1}{2}\bigg[\ln|u|\bigg]_3^{15}    & \\
              & = \dfrac{1}{2}(\ln 15 - \ln 3)             & \\
              & = \dfrac{1}{2}\ln 5
        \end{flalign*}
    \end{multicols}

    \begin{multicols}{2}
        \item $\displaystyle\int_{-1}^3 \sqrt{2 x+3} d x$
        \sol{}

        Let $u = 2x + 3$, $du = 2dx$.

        When $x = -1$, $u = 1$.

        When $x = 3$, $u = 9$.
        \begin{flalign*}
            I & = \dfrac{1}{2}\int_1^9 \sqrt{u} d u           & \\
              & = \dfrac{1}{3}\bigg[u^{\frac{3}{2}}\bigg]_1^9 & \\
              & = \dfrac{1}{3}(27 - 1)                        & \\
              & = \dfrac{26}{3}
        \end{flalign*}

        \item $\displaystyle\int_1^2 \dfrac{1}{(2 x-1)^3} d x$
        \sol{}

        Let $u = 2x - 1$, $du = 2dx$.

        When $x = 1$, $u = 1$.

        When $x = 2$, $u = 3$.
        \begin{flalign*}
            I & = \dfrac{1}{2}\int_1^3 u^{-3} d u                & \\
              & = -\dfrac{1}{4}\bigg[u^{-2}\bigg]_1^3            & \\
              & = -\dfrac{1}{4}\left(\dfrac{1}{9} - 1\right)     & \\
              & = -\dfrac{1}{4} \cdot \left(-\dfrac{8}{9}\right) & \\
              & = \dfrac{2}{9}
        \end{flalign*}
    \end{multicols}

    \begin{multicols}{2}
        \item $\displaystyle\int_{-1}^1 x^2\left(x^3-1\right)^4 d x$
        \sol{}

        Let $u = x^3 - 1$, $du = 3x^2dx$.

        When $x = -1$, $u = -2$.

        When $x = 1$, $u = 0$.
        \begin{flalign*}
            I & = \dfrac{1}{3}\int_{-2}^0 u^4 d u     & \\
              & = \dfrac{1}{15}\bigg[u^5\bigg]_{-2}^0 & \\
              & = \dfrac{32}{15}
        \end{flalign*}
        \columnbreak{}

        \item $\displaystyle\int_1^6 x \sqrt{3 x-2} d x$
        \sol{}

        Let $u = 3x - 2$, $du = 3dx$, $x = \dfrac{u + 2}{3}$.

        When $x = 1$, $u = 1$.

        When $x = 6$, $u = 16$.
        \begin{flalign*}
            I & = \dfrac{1}{3}\int_1^{16} \dfrac{u + 2}{3}\sqrt{u} d u                                     & \\
              & = \dfrac{1}{9}\int_1^{16} \left(u^{\frac{3}{2}} + 2u^{\frac{1}{2}}\right) d u              & \\
              & = \dfrac{1}{9}\bigg[\dfrac{2}{5}u^{\frac{5}{2}} + \dfrac{4}{3}u^{\frac{3}{2}}\bigg]_1^{16} & \\
              & = \dfrac{1}{9}\left(\dfrac{2048}{5} + \dfrac{256}{3} - \dfrac{2}{5} - \dfrac{4}{3}\right)  & \\
              & = \dfrac{274}{5}
        \end{flalign*}
    \end{multicols}

    \newpage
    \item $\displaystyle\int_{-\frac{\pi}{4}}^{\frac{\pi}{4}} \sin ^2 \theta d \theta$
          \sol{}
          \begin{flalign*}
              I & = \dfrac{1}{2}\int_{-\frac{\pi}{4}}^{\frac{\pi}{4}} (1 - \cos 2\theta) d \theta              & \\
                & = \dfrac{1}{2}\bigg[\theta - \dfrac{1}{2}\sin 2\theta\bigg]_{-\frac{\pi}{4}}^{\frac{\pi}{4}} & \\
                & = \dfrac{1}{2}\left(\dfrac{\pi}{4} - \dfrac{1}{2} + \dfrac{\pi}{4} - \dfrac{1}{2}\right)     & \\
                & = \dfrac{\pi}{4} - \dfrac{1}{2}                                                              & \\
                & = \dfrac{\pi - 2}{4}
          \end{flalign*}

    \item $\displaystyle\int_3^5 \dfrac{1}{x^2-x-2} d x$
          \sol{}
          \begin{flalign*}
              I & = \int_3^5 \dfrac{1}{(x-2)(x+1)} d x &
          \end{flalign*}
          Let $\dfrac{1}{(x-2)(x+1)} = \dfrac{A}{x-2} + \dfrac{B}{x+1}$.
          \begin{flalign*}
              Ax + A + Bx - 2B    & = 1 \\
              (A + B)x + (A - 2B) & = 1
          \end{flalign*}
          \vspace{-2em}
          \begin{flalign*}
              \begin{cases}
                  A + B = 0 \\
                  A - 2B = 1
              \end{cases}
              \Rightarrow
              \begin{cases}
                  A = \dfrac{1}{3} \\
                  B = -\dfrac{1}{3}
              \end{cases}
          \end{flalign*}
          \vspace{-1em}
          \begin{flalign*}
              I & = \int_3^5 \left(\dfrac{1}{3(x-2)} - \dfrac{1}{3(x+1)}\right) d x       & \\
                & = \dfrac{1}{3}\int_3^5 \left(\dfrac{1}{x-2} - \dfrac{1}{x+1}\right) d x & \\
                & = \dfrac{1}{3}\bigg[\ln|x-2| - \ln|x+1|\bigg]_3^5                       & \\
                & = \dfrac{1}{3}\left(\ln 3 - \ln 6 - \ln 1 + \ln 4\right)                & \\
                & = \dfrac{1}{3}\ln 2
          \end{flalign*}

          \newpage

          \begin{multicols}{2}
              \item $\displaystyle\int_2^5 \dfrac{x}{x^3-x^2-x+1} d x$
              \sol{}
              \begin{flalign*}
                  I & = \int_2^5 \dfrac{x}{x^2(x-1) - (x-1)} d x & \\
                    & = \int_2^5 \dfrac{x}{(x^2 - 1)(x-1)} d x   & \\
                    & = \int_2^5 \dfrac{x}{(x + 1)(x-1)^2} d x
              \end{flalign*}
              Let $\dfrac{x}{(x + 1)(x-1)^2} = \dfrac{A}{x+1} + \dfrac{B}{x-1} + \dfrac{C}{(x-1)^2}$.
              \begin{flalign*}
                  Ax^2 - 2Ax + A + Bx^2 - B + Cx + C    & = x & \\
                  (A + B)x^2 + (-2A + C)x + (A - B + C) & = x
              \end{flalign*}
              \vspace{-2em}
              \begin{flalign*}
                  \begin{cases}
                      A + B = 0   \\
                      -2A + C = 1 \\
                      A - B + C = 0
                  \end{cases}
                  \Rightarrow
                  \begin{cases}
                      A = -\dfrac{1}{4} \\
                      B = \dfrac{1}{4}  \\
                      C = \dfrac{1}{2}
                  \end{cases}
              \end{flalign*}
              \vspace{-1em}
              \begin{flalign*}
                  I & = \int_2^5 \left(-\dfrac{1}{4(x+1)} + \dfrac{1}{4(x-1)} + \dfrac{1}{2(x-1)^2}\right) d x                       & \\
                    & = \left[-\dfrac{1}{4}\ln|x+1| + \dfrac{1}{4}\ln|x-1| - \dfrac{1}{2(x-1)}\right]_2^5                            & \\
                    & = -\dfrac{1}{4}\ln 6 + \dfrac{1}{4}\ln 4 - \dfrac{1}{8} + \dfrac{1}{4}\ln 3 - \dfrac{1}{4}\ln 1 + \dfrac{1}{2} & \\
                    & = -\dfrac{1}{4}\ln 6 + \dfrac{1}{4}\ln 4 - \dfrac{1}{8} + \dfrac{1}{4}\ln 3 + \dfrac{1}{2}                     & \\
                    & = \dfrac{1}{4}\ln 2 + \dfrac{3}{8}
              \end{flalign*}

              \item $\displaystyle\int_0^1 \dfrac{x^2}{x^2+2 x+1} d x$
              \sol{}
              \begin{flalign*}
                  I & = \int_0^1 \dfrac{x^2}{(x+1)^2} d x &
              \end{flalign*}
              Let $u = x + 1$, $du = dx$, $x = u - 1$.

              When $x = 0$, $u = 1$.

              When $x = 1$, $u = 2$.
              \begin{flalign*}
                  I & = \int_1^2 \dfrac{(u - 1)^2}{u^2} d u                         & \\
                    & = \int_1^2 \dfrac{u^2 - 2u + 1}{u^2} d u                      & \\
                    & = \int_1^2 \left(1 - \dfrac{2}{u} + \dfrac{1}{u^2}\right) d u & \\
                    & = \bigg[u - 2\ln|u| - \dfrac{1}{u}\bigg]_1^2                  & \\
                    & = 2 - 2\ln 2 - \dfrac{1}{2} - 1 + 2\ln 1 + 1                  & \\
                    & = \dfrac{3}{2} - 2\ln 2
              \end{flalign*}
          \end{multicols}

          \begin{multicols}{2}
              \item $\displaystyle\int_0^3 \dfrac{x}{\sqrt{25-x^2}} d x$
              \sol{}

              Let $u = 25 - x^2$, $du = -2xdx$.

              When $x = 0$, $u = 25$.

              When $x = 3$, $u = 16$.
              \begin{flalign*}
                  I & = \dfrac{1}{2}\int_{16}^{25} \dfrac{1}{\sqrt{u}} d u & \\
                    & = \bigg[\sqrt{u}\bigg]_{16}^{25}                     & \\
                    & = 5 - 4                                              & \\
                    & = 1
              \end{flalign*}

              \item $\displaystyle\int_0^{\frac{\pi}{6}} \sin ^2 \theta \cos \theta d \theta$
              \sol{}

              Let $u = \sin \theta$, $du = \cos \theta d \theta$.

              When $\theta = 0$, $u = 0$.

              When $\theta = \dfrac{\pi}{6}$, $u = \dfrac{1}{2}$.
              \begin{flalign*}
                  I & = \int_0^{\frac{1}{2}} u^2 d u                & \\
                    & = \bigg[\dfrac{1}{3}u^3\bigg]_0^{\frac{1}{2}} & \\
                    & = \dfrac{1}{24}
              \end{flalign*}
          \end{multicols}

          \newpage
    \item Given that $f(x)=\left\{\begin{array}{cc}2 x^2-1, & -2 \leq x \leq 2 \\ 3 x+1, & 2<x \leq 4\end{array}\right.$, find $\displaystyle\int_{-2}^4 f(x) d x$.
          \sol{}
          \begin{flalign*}
              I & = \int_{-2}^2 (2x^2 - 1) d x + \int_2^4 (3x + 1) d x                           & \\
                & = \bigg[\dfrac{2}{3}x^3 - x\bigg]_{-2}^2 + \bigg[\dfrac{3}{2}x^2 + x\bigg]_2^4 & \\
                & = \dfrac{16}{3} - 2 + \dfrac{16}{3} - 2 + 24 + 4 - 6 - 2                       & \\
                & = \dfrac{80}{3}
          \end{flalign*}

    \item Given that $\displaystyle\int_3^5 f(x) d x=6, \int_5^9 f(x) d x=18, \int_1^4
              g(x) d x=4$ and $\displaystyle\int_3^4 g(x) d x=-4$. Find:
          \begin{enumerate}
              \item $\displaystyle\int_1^3 g(x) d x$;
                    \sol{}
                    \begin{flalign*}
                        \int_1^3 g(x) d x & = \int_1^4 g(x) d x - \int_3^4 g(x) d x & \\
                                          & = 4 - (-4)                              & \\
                                          & = 8
                    \end{flalign*}

              \item $\displaystyle\int_1^3 f(3 x) d x$;
                    \sol{}

                    Let $u = 3x$, $du = 3dx$.

                    When $x = 1$, $u = 3$.

                    When $x = 3$, $u = 9$.
                    \begin{flalign*}
                        \int_1^3 f(3 x) d x & = \dfrac{1}{3}\int_3^9 f(u) d u                                 & \\
                                            & = \dfrac{1}{3}\int_3^5 f(u) d u + \dfrac{1}{3}\int_5^9 f(u) d u & \\
                                            & = \dfrac{1}{3}(6 + 18)                                          & \\
                                            & = 8
                    \end{flalign*}

              \item $\displaystyle\int_1^3[f(3 x)-3 g(x)] d x$.
                    \sol{}
                    \begin{flalign*}
                        \int_1^3[f(3 x)-3 g(x)] d x & = \int_1^3 f(3 x) d x - 3\int_1^3 g(x) d x & \\
                                                    & = 8 - 3 \cdot 8                            & \\
                                                    & = -16
                    \end{flalign*}
          \end{enumerate}
          \newpage

          \begin{multicols}{2}
              \item Given the function $y=x \sqrt{x+1}$, \\find $\dfrac{d y}{d x}$. Hence, find
              $\displaystyle\int_3^8 \dfrac{3 x+2}{\sqrt{x+1}} d x$. \sol{}
              \begin{flalign*}
                  \dfrac{d y}{d x}                       & = \sqrt{x + 1} + \dfrac{x}{2\sqrt{x + 1}}  & \\
                                                         & = \dfrac{2x + x + 2}{2\sqrt{x + 1}}        & \\
                                                         & = \dfrac{3x + 2}{2\sqrt{x + 1}}            & \\
                  \\
                  \int_3^8 \dfrac{3 x+2}{\sqrt{x+1}} d x & = 2\int_3^8 \dfrac{3 x+2}{2\sqrt{x+1}} d x & \\
                                                         & = 2\int_3^8 \dfrac{d y}{d x} d x           & \\
                                                         & = 2\left[x \sqrt{x + 1}\right]_3^8         & \\
                                                         & = 2\left(24 - 6\right)                     & \\
                                                         & = 36
              \end{flalign*}
              \vfill{}\null{}

              \item Given the function $y=\dfrac{x^2-1}{2 x+1}$, \\find $\dfrac{d y}{d x}$. Hence,
              find $\displaystyle\int_0^2 \dfrac{x^2+x+1}{4 x^2+4 x+1} d x$. \sol{}
              \begin{flalign*}
                  \dfrac{d y}{d x}                          & = \dfrac{(2x + 1)(2x) - (x^2 - 1)(2)}{(2x + 1)^2}             & \\
                                                            & = \dfrac{4x^2 + 2x - 2x^2 + 2}{(2x + 1)^2}                    & \\
                                                            & = \dfrac{2(x^2 + x + 1)}{(2x + 1)^2}                          & \\
                  \\
                  \int_0^2 \dfrac{x^2+x+1}{4 x^2+4 x+1} d x & = \dfrac{1}{2}\int_0^2 \dfrac{2(x^2 + x + 1)}{(2x + 1)^2} d x & \\
                                                            & = \dfrac{1}{2}\int_0^2 \dfrac{d y}{d x} d x                   & \\
                                                            & = \dfrac{1}{2}\left[\dfrac{x^2 - 1}{2x + 1}\right]_0^2        & \\
                                                            & = \dfrac{1}{2}\left(\dfrac{3}{5} - \dfrac{-1}{1}\right)       & \\
                                                            & = \dfrac{4}{5}
              \end{flalign*}
              \vfill\null{}
          \end{multicols}

    \item Given the function $y=x e^x-e^x$, find $\dfrac{d y}{d x}$. Hence, find
          $\displaystyle\int_1^4 2 x e^x d x$. \sol{}
          \begin{flalign*}
              \dfrac{d y}{d x}     & = x e^x + e^x - e^x                & \\
                                   & = x e^x                            & \\
              \\
              \int_1^4 2 x e^x d x & = 2\int_1^4 x e^x d x              & \\
                                   & = 2\int_1^4 \dfrac{d y}{d x} d x   & \\
                                   & = 2\left[x e^x - e^x\right]_1^4    & \\
                                   & = 2\left(4e^4 - e^4 - e + e\right) & \\
                                   & = 6e^4
          \end{flalign*}
\end{enumerate}

\newpage
