\documentclass{report}
\usepackage[a4paper,total={7in,10in}]{geometry}

\usepackage{amsmath}
\usepackage{amssymb}
\usepackage{enumitem}

\setcounter{chapter}{10}
\setcounter{section}{2}

\newcommand{\sol}{\vspace{1em}\\\textbf{Sol.}}
\newcommand{\eos}{ \qquad \square}

\begin{document}
\section*{Exercise 5a}

\begin{enumerate}[leftmargin=*]
    \item Given that the coordinates of a fixed point are $(-1, 2)$, the equation of a
          fixed line is $x - y + 4 = 0$, the ratio of the distance between a moving point
          and the fixed point to the distance between the moving point and the fixed line
          is $\dfrac{\sqrt{2}}{2}$. Explain the graph of the locus of the moving point
          $P$. Hence, find its equation. \sol{}

          From the definition of conic section, the locus of the moving point $P$ is a
          conic section. Since the ratio is $\dfrac{\sqrt{2}}{2}$, the eccentricity is
          smaller than 1, so the conic section is an ellipse.

          Let the coordinates of the moving point $P$ be $(x, y)$, we have
          \begin{flalign*}
              \frac{\sqrt{(x + 1)^2 + (y - 2)^2}}{\left|\dfrac{x - y + 4}{\sqrt{2}}\right|} & = \frac{\sqrt{2}}{2}             & \\
              \frac{(x + 1)^2 + (y - 2)^2}{\dfrac{(x - y + 4)^2}{2}}                        & = \frac{1}{2}                    & \\
              4(x + 1)^2 + 4(y - 2)^2                                                       & = (x - y + 4)^2                  & \\
              4(x^2 + 2x + 1) + 4(y^2 - 4y + 4)                                             & = x^2 + y^2 + 16 - 2xy + 8x - 8y & \\
              4x^2 + 8x + 4 + 4y^2 - 16y + 16                                               & = x^2 + y^2 + 16 - 2xy + 8x - 8y & \\
              3x^2 + 3y^2 + 2xy - 8y + 4                                                    & = 0    \eos
          \end{flalign*}

    \item The distance from a moving point $P$ and the point $A(0, 2)$ is equal to the
          distance between $P$ and the $x$-axis. Find the equation of the locus of $P$.
          \sol{}
          \begin{flalign*}
              \sqrt{x^2 + (y - 2)^2} & = y         & \\
              x^2 + (y - 2)^2        & = y^2       & \\
              x^2 + y^2 - 4y + 4     & = y^2       & \\
              x^2 - 4y + 4           & = 0    \eos
          \end{flalign*}
    \item Given the coordinates of the focus point, the equation of the directrix, and
          the eccentricity of a conic section, find the equation of the conic section:
          \begin{enumerate}
              \item $(1, 1)$, $x-y-1=0$, $e=1$
                    \sol{}
                    \begin{flalign*}
                        \frac{\sqrt{(x - 1)^2 + (y - 1)^2}}{\left|\dfrac{x - y - 1}{\sqrt{2}}\right|} & = 1                             & \\
                        \frac{(x - 1)^2 + (y - 1)^2}{(x - y - 1)^2}                                   & = \frac{1}{2}                   & \\
                        2(x - 1)^2 + 2(y - 1)^2                                                       & = (x - y - 1)^2                 & \\
                        2(x^2 - 2x + 1) + 2(y^2 - 2y + 1)                                             & = x^2 + y^2 + 1 - 2xy - 2x + 2y & \\
                        2x^2 - 4x + 2 + 2y^2 - 4y + 2                                                 & = x^2 + y^2 + 1 - 2xy - 2x + 2y & \\
                        x^2 + y^2 + 2xy - 2x - 6y + 3                                                 & = 0    \eos
                    \end{flalign*}
                    \newpage
              \item $(1, 0)$, $2x+y=0$, $e=1$
                    \sol{}
                    \begin{flalign*}
                        \frac{\sqrt{(x - 1)^2 + y^2}}{\left|\dfrac{2x + y}{\sqrt{5}}\right|} & = 1                & \\
                        \frac{(x - 1)^2 + y^2}{\dfrac{(2x + y)^2}{5}}                        & = 1                & \\
                        5(x - 1)^2 + 5y^2                                                    & = (2x + y)^2       & \\
                        5(x^2 - 2x + 1) + 5y^2                                               & = 4x^2 + 4xy + y^2 & \\
                        5x^2 - 10x + 5 + 5y^2                                                & = 4x^2 + 4xy + y^2 & \\
                        x^2 - y^2 - 4xy - 10x + 5                                            & = 0    \eos
                    \end{flalign*}
              \item $(2, 0)$, $x=0$, $e=1$
                    \sol{}
                    \begin{flalign*}
                        \frac{\sqrt{(x - 2)^2 + y^2}}{\left|\dfrac{x}{\sqrt{2}}\right|} & = 1        & \\
                        \frac{(x - 2)^2 + y^2}{\dfrac{x^2}{2}}                          & = 1        & \\
                        2(x - 2)^2 + 2y^2                                               & = x^2      & \\
                        2(x^2 - 4x + 4) + 2y^2                                          & = x^2      & \\
                        2x^2 - 8x + 8 + 2y^2                                            & = x^2      & \\
                        2y^2 - 8x + 8                                                   & = 0        & \\
                        y^2 - 4x + 4                                                    & = 0   \eos
                    \end{flalign*}
              \item $(0, 0)$, $3x + 3y + 1 = 0$, $e = \dfrac{2}{3}$
                    \sol{}
                    \begin{flalign*}
                        \frac{\sqrt{x^2 + y^2}}{\left|\dfrac{3x + 3y + 1}{\sqrt{18}}\right|} & = \frac{2}{3}                          & \\
                        \frac{x^2 + y^2}{\dfrac{(3x + 3y + 1)^2}{18}}                        & = \frac{4}{9}                          & \\
                        81(x^2 + y^2)                                                        & = 2(3x + 3y + 1)^2                     & \\
                        81x^2 + 81y^2                                                        & = 2(9x^2 + 18xy + 9y^2 + 6x + 6y + 1)  & \\
                        81x^2 + 81y^2                                                        & = 18x^2 + 36xy + 18y^2 + 12x + 12y + 2 & \\
                        63x^2 + 63y^2                                                        & - 36xy - 12x - 12y - 2 = 0 \eos
                    \end{flalign*}
                    \newpage
              \item $(-4, 0)$, $y + 3 = 0$, $e = \dfrac{1}{4}$
                    \sol{}
                    \begin{flalign*}
                        \frac{\sqrt{(x + 4)^2 + y^2}}{\left|\dfrac{y + 3}{\sqrt{1}}\right|} & = \frac{1}{4}  & \\
                        \frac{(x + 4)^2 + y^2}{(y + 3)^2}                                   & = \frac{1}{16} & \\
                        16(x + 4)^2 + 16y^2                                                 & = (y + 3)^2    & \\
                        16(x^2 + 8x + 16) + 16y^2                                           & = y^2 + 6y + 9 & \\
                        16x^2 + 128x + 256 + 16y^2                                          & = y^2 + 6y + 9 & \\
                        16x^2 + 15y^2 + 128x - 6y + 247                                     & = 0    \eos
                    \end{flalign*}
              \item $(1, 2)$, $x + y + 1 = 0$, $e = 2$
                    \sol{}
                    \begin{flalign*}
                        \frac{\sqrt{(x - 1)^2 + (y - 2)^2}}{\left|\dfrac{x + y + 1}{\sqrt{2}}\right|} & = 2                                & \\
                        \frac{(x - 1)^2 + (y - 2)^2}{\dfrac{(x + y + 1)^2}{2}}                        & = 4                                & \\
                        (x - 1)^2 + (y - 2)^2                                                         & = 2(x + y + 1)^2                   & \\
                        x^2 - 2x + 1 + y^2 - 4y + 4                                                   & = 2(x^2 + y^2 + 1 + 2xy + 2x + 2y) & \\
                        x^2 - 2x + 1 + y^2 - 4y + 4                                                   & = 2x^2 + 2y^2 + 2 + 4xy + 4x + 4y  & \\
                        x^2 + y^2 + 4xy + 6x + 8y - 3                                                 & = 0    \eos
                    \end{flalign*}
              \item $(0, -1)$, $x + 2y - 1 = 0$, $e = \sqrt{3}$
                    \sol{}
                    \begin{flalign*}
                        \frac{\sqrt{x^2 + (y + 1)^2}}{\left|\dfrac{x + 2y - 1}{\sqrt{5}}\right|} & = \sqrt{3}                           & \\
                        \frac{x^2 + (y + 1)^2}{\dfrac{(x + 2y - 1)^2}{5}}                        & = 3                                  & \\
                        5x^2 + 5(y + 1)^2                                                        & = 3(x + 2y - 1)^2                    & \\
                        5x^2 + 5(y^2 + 2y + 1)                                                   & = 3(x^2 + 4xy - 2x + 4y^2 - 4y + 1)  & \\
                        5x^2 + 5y^2 + 10y + 5                                                    & = 3x^2 + 12xy - 6x + 12y^2 - 12y + 3 & \\
                        2x^2 - 7y^2 - 12xy + 6x                                                  & + 22y + 2 = 0    \eos
                    \end{flalign*}
          \end{enumerate}
\end{enumerate}
\end{document}