\subsection{Exercise 27.3b}
\noindent \hspace{1.2em}\textit{Find the following indefinite integral:}
\begin{enumerate}
    \begin{multicols}{2}
        \item $\displaystyle\int\sin^2\dfrac{x}{2} dx$
        \sol{}
        \begin{flalign*}
            I & = \int\left(\dfrac{1 - \cos x}{2}\right) dx       & \\
              & = \dfrac{1}{2}\int dx - \dfrac{1}{2}\int\cos x dx & \\
              & = \dfrac{1}{2}x - \dfrac{1}{2}\sin x + C
        \end{flalign*}
        \vfill{}\null{}

        \item $\displaystyle\int\tan^2 5x dx$
        \sol{}
        \begin{flalign*}
            I & = \int\left(\sec^2 5x - 1\right) dx        & \\
              & = \int\sec^2 5x dx - \int dx               & \\
              & = \dfrac{1}{5}\int\sec^2 5xd(5x) - \int dx & \\
              & = \dfrac{1}{5}\tan 5x - x + C
        \end{flalign*}
    \end{multicols}

    \begin{multicols}{2}
        \item $\displaystyle\int\dfrac{1}{\sec^2 4x} dx$
        \sol{}
        \begin{flalign*}
            I & = \int\cos^2 4x dx                                 & \\
              & = \int\dfrac{1 + \cos 8x}{2} dx                    & \\
              & = \dfrac{1}{2}\int dx + \dfrac{1}{2}\int\cos 8x dx & \\
              & = \dfrac{1}{16}\sin 8x + \dfrac{1}{2}x + C
        \end{flalign*}

        \item $\displaystyle\int\cos^2(3x - 1) dx$
        \sol{}
        \begin{flalign*}
            I & = \int\left(\dfrac{1 + \cos 2(3x - 1)}{2}\right) dx      & \\
              & = \dfrac{1}{2}\int dx + \dfrac{1}{2}\int\cos (6x - 2) dx & \\
              & = \dfrac{1}{12}\sin (6x - 2) + \dfrac{1}{2}x + C
        \end{flalign*}
    \end{multicols}

    \begin{multicols}{2}
        \item $\displaystyle\int\sec5x\tan5x dx$
        \sol{}
        \begin{flalign*}
            I & = \dfrac{1}{5}\int\sec5x\tan5x d(5x) & \\
              & = \dfrac{1}{5}\sec5x + C
        \end{flalign*}

        \item $\displaystyle\int-\csc3x\cot3x dx$
        \sol{}
        \begin{flalign*}
            I & = \dfrac{1}{3}\int-\csc3x\cot3x d(3x) & \\
              & = \dfrac{1}{3}\csc3x + C
        \end{flalign*}
    \end{multicols}

    \begin{multicols}{2}
        \item $\displaystyle\int\left(\sin\dfrac{x}{8} - \sec^2 2x\right) dx$
        \sol{}
        \begin{flalign*}
            I & = \int\sin\dfrac{x}{8} dx - \int\sec^2 2x dx                                           & \\
              & = -8\int\sin \dfrac{x}{8} d\left(\dfrac{x}{8}\right) - \dfrac{1}{2}\int\sec^2 2x d(2x) & \\
              & = -8\cos\dfrac{x}{8} - \dfrac{1}{2}\tan 2x + C
        \end{flalign*}
        \vfill{}\null{}
        \columnbreak{}

        \item $\displaystyle\int\left(\sin{\dfrac{x}{2}}+\cos{\dfrac{x}{2}}\right)^{2} dx$
        \sol{}

        Let $u = \dfrac{x}{2}$, $du = \dfrac{1}{2}dx$.
        \begin{flalign*}
            I & = 2\int\left(\sin u + \cos u\right)^2 du                   & \\
              & = 2\int\left(\sin^2 u + 2\sin u\cos u + \cos^2 u\right) du & \\
              & = 2\int\left(1 + \sin 2u\right) du                         & \\
              & = 2\left(u - \dfrac{1}{2}\cos 2u\right) + C                & \\
              & = x - \cos x + C
        \end{flalign*}
    \end{multicols}

    \begin{multicols}{2}
        \item $\displaystyle\int(\sec x+\tan x)^{2} dx$
        \sol{}
        \begin{flalign*}
            I & = \int(\sec^2 x + 2\sec x\tan x + \tan^2 x) dx                   & \\
              & = \int\sec^2 x + 2\int\sec x\tan x dx + \int\tan^2 x dx          & \\
              & = \int\sec^2 x dx + 2\int\sec x\tan x dx + \int(\sec^2 x - 1) dx & \\
              & = \tan x + 2\sec x + \tan x - x + C                              & \\
              & = 2\tan x + 2\sec x - x + C
        \end{flalign*}

        \item $\displaystyle\int(2-\sin x)^{2} dx$
        \sol{}
        \begin{flalign*}
            I & = \int(4 - 4\sin x + \sin^2 x) dx                                               & \\
              & = \int 4 dx - 4\int\sin x dx + \dfrac{1}{2}\int(1 - \cos 2x) dx                 & \\
              & = \int 4 dx - 4\int\sin x dx + \dfrac{1}{2}\int dx - \dfrac{1}{2}\int\cos 2x dx & \\
              & = 4x + 4\cos x + \dfrac{1}{2}x - \dfrac{1}{4}\sin 2x + C                        & \\
              & = \dfrac{9}{2}x + 4\cos x - \dfrac{1}{4}\sin 2x + C
        \end{flalign*}
    \end{multicols}

    \begin{multicols}{2}
        \item $\displaystyle\int\cos^4 x dx$
        \sol{}
        \begin{flalign*}
            I & = \int\cos^2 x\cos^2 x dx                                                                         & \\
              & = \int(1 - \sin^2 x)\cos^2 x dx                                                                   & \\
              & = \int\cos^2 x dx - \int\sin^2 x\cos^2 x dx                                                       & \\
              & = \int\dfrac{1 + \cos 2x}{2} dx - \int\dfrac{1 - \cos 2x}{2}\cdot\dfrac{1 + \cos 2x}{2} dx        & \\
              & = \dfrac{1}{2}\int dx + \dfrac{1}{2}\int\cos 2x dx - \dfrac{1}{4}\int(1 - \cos^2 2x) dx           & \\
              & = \dfrac{1}{2}\int dx + \dfrac{1}{2}\int\cos 2x dx - \dfrac{1}{4}\int dx                          & \\
              & \ \ \ \ + \dfrac{1}{4}\int\dfrac{1 + \cos 4x}{2} dx                                               & \\
              & = \dfrac{1}{2}\int dx + \dfrac{1}{2}\int\cos 2x dx - \dfrac{1}{4}\int dx + \dfrac{1}{8}\int dx    & \\
              & \ \ \ \ + \dfrac{1}{8}\int\cos 4x dx                                                              & \\
              & = \dfrac{1}{2}x + \dfrac{1}{4}\sin 2x - \dfrac{1}{4}x + \dfrac{1}{16}x + \dfrac{1}{32}\sin 4x + C & \\
              & = \dfrac{3}{8}x + \dfrac{1}{4}\sin 2x + \dfrac{1}{32}\sin 4x + C
        \end{flalign*}

        \item $\displaystyle\int\left(1+\tan^{2}x\right)\left(1-\tan^{2}x\right) dx$
        \sol{}
        \begin{flalign*}
            I & = \int\left(1 - \tan^4 x\right) dx                              & \\
              & = \int dx - \int\tan^4 x dx                                     & \\
              & = \int dx - \int(\sec^2 x - 1)\tan^2 x dx                       & \\
              & = \int dx - \int\sec^2 x\tan^2 x dx + \int\tan^2 x dx           & \\
              & = \int dx - \int\sec^2 x\tan^2 x dx + \int(\sec^2 x - 1)dx      & \\
              & = \int dx - \int\sec^2 x\tan^2 x dx + \int\sec^2 x dx - \int dx & \\
              & = \int\sec^2 x dx - \int\sec^2 x\tan^2 x dx
        \end{flalign*}
        Let $u = \tan x$, $du = \sec^2 xdx$.
        \begin{flalign*}
            I & = \int\sec ^{2}x dx - \int u^{2}du  & \\
              & = \tan x - \dfrac{u^{3}}{3} + C     & \\
              & = \tan x - \dfrac{\tan^{3}x}{3} + C
        \end{flalign*}
    \end{multicols}

    \begin{multicols}{2}
        \item $\displaystyle\int\sin^{2}4x\cos4x dx$
        \sol{}

        Let $u = \sin 4x$, $du = 4\cos 4x dx$.
        \begin{flalign*}
            I & = \dfrac{1}{4}\int u^2 du             & \\
              & = \dfrac{1}{4}\cdot\dfrac{u^3}{3} + C & \\
              & = \dfrac{1}{12}\sin^3 4x + C
        \end{flalign*}

        \item $\displaystyle\int3\cot^{3}3x\csc^{2}3x dx$
        \sol{}

        Let $u = \cot 3x$, $du = -3\csc^2 3x dx$.
        \begin{flalign*}
            I & = -\int u^3 du               & \\
              & = -\dfrac{u^4}{4} + C        & \\
              & = -\dfrac{1}{4}\cot^4 3x + C
        \end{flalign*}
    \end{multicols}

    \begin{multicols}{2}
        \item $\displaystyle\int\tan^{2}x\sec^{4}x dx$
        \sol{}
        \begin{flalign*}
            I & = \int\tan^{2}x(\tan^2 x + 1)\sec^2 x dx            & \\
              & = \int\tan^4 x\sec^2 x dx + \int\tan^2 x\sec^2 x dx
        \end{flalign*}
        Let $u = \tan x$, $du = \sec^2 xdx$.
        \begin{flalign*}
            I & = \int u^4 du + \int u^2 du                       & \\
              & = \dfrac{u^5}{5} + \dfrac{u^3}{3} + C             & \\
              & = \dfrac{1}{5}\tan^5 x + \dfrac{1}{3}\tan^3 x + C
        \end{flalign*}

        \item $\displaystyle\int\sec x\cdot\tan^{3}x dx$
        \sol{}
        \begin{flalign*}
            I & = \int\sec x\cdot(\sec^2 x - 1)\tan x dx      & \\
              & = \int\sec^3 x\tan x dx - \int\sec x\tan x dx
        \end{flalign*}
        Let $u = \sec x$, $du = \sec x\tan xdx$.
        \begin{flalign*}
            I & = \int u^2 du - \int \sec x\tan xdx & \\
              & = \dfrac{u^3}{3} - \sec x + C       & \\
              & = \dfrac{1}{3}\sec^3 x - \sec x + C
        \end{flalign*}
    \end{multicols}
\end{enumerate}