\subsection{Exercise 27.2b}
Find the following indefinite integrals (Question 1 to 20):
\begin{enumerate}
    \begin{multicols}{2}
        \item $\displaystyle\int(x^3 - 3x + 1)dx$
        \sol{}
        \begin{flalign*}
            I & = \int x^3dx - \int 3xdx + \int dx          & \\
              & = \dfrac{1}{4}x^4 - \dfrac{3}{2}x^2 + x + C
        \end{flalign*}

        \item $\displaystyle\int\left(5x^4 + 2\sqrt{x}\right)dx$
        \sol{}
        \begin{flalign*}
            I & = \int 5x^4dx + \int 2\sqrt{x}dx        & \\
              & = x^5 + \dfrac{4}{3}x^{\frac{3}{2}} + C
        \end{flalign*}
    \end{multicols}

    \begin{multicols}{2}
        \item $\displaystyle\int\left({\dfrac{x^{2}}{2}}-{\dfrac{2}{x^{2}}}\right)dx$
        \sol{}
        \begin{flalign*}
            I & = \int{\dfrac{x^{2}}{2}}dx - \int{\dfrac{2}{x^{2}}}dx & \\
              & = \dfrac{1}{6}x^{3} + \dfrac{2}{x} + C
        \end{flalign*}
        \vfill{}\null{}

        \item $\displaystyle\int(\sin x-3\cos x)dx$
        \sol{}
        \begin{flalign*}
            I & = \int\sin xdx - \int3\cos xdx & \\
              & = -\cos x - 3\sin x + C
        \end{flalign*}
        \vfill{}\null{}
    \end{multicols}
    \vspace{-4em}
    \begin{multicols}{2}
        \item $\displaystyle\int(x-5)^2dx$
        \sol{}
        \begin{flalign*}
            I & = \int(x^2 - 10x + 25)dx           & \\
              & = \dfrac{1}{3}x^3 - 5x^2 + 25x + C
        \end{flalign*}

        \item $\displaystyle\int(x-1)(x-2)dx$
        \sol{}
        \begin{flalign*}
            I & = \int(x^2 - 3x + 2)dx                       & \\
              & = \dfrac{1}{3}x^3 - \dfrac{3}{2}x^2 + 2x + C
        \end{flalign*}
    \end{multicols}

    \begin{multicols}{2}
        \item $\displaystyle\int(x^2 + 2)\sqrt{x}dx$
        \sol{}
        \begin{flalign*}
            I & = \int x^{\frac{5}{2}}dx + \int 2x^{\frac{1}{2}}dx              & \\
              & = \dfrac{2}{7}x^{\frac{7}{2}} + \dfrac{4}{3}x^{\frac{3}{2}} + C
        \end{flalign*}

        \item $\displaystyle\int\dfrac{x^4 - 5}{x^2}dx$
        \sol{}
        \begin{flalign*}
            I & = \int x^2dx - \int\dfrac{5}{x^2}dx  & \\
              & = \dfrac{1}{3}x^3 + \dfrac{5}{x} + C
        \end{flalign*}
    \end{multicols}

    \begin{multicols}{2}
        \item $\displaystyle\int\dfrac{x+5}{\sqrt{x}}dx$
        \sol{}
        \begin{flalign*}
            I & = \int x^{\frac{1}{2}}dx + \int 5x^{-\frac{1}{2}}dx   & \\
              & = \dfrac{2}{3}x^{\frac{3}{2}} + 10x^{\frac{1}{2}} + C
        \end{flalign*}
        \vfill{}\null{}

        \item $\displaystyle\int\dfrac{\sqrt[3]{x^2} - \sqrt[4]{x}}{\sqrt{x}}dx$
        \sol{}
        \begin{flalign*}
            I & = \int \dfrac{x^{\frac{2}{3}} - x^{\frac{1}{4}}}{x^{\frac{1}{2}}}dx & \\
              & = \int \left(x^{\frac{1}{6}} - x^{-\frac{1}{4}}\right)dx            & \\
              & = \dfrac{6}{7}x^{\frac{7}{6}} - \dfrac{4}{3}x^{\frac{3}{4}} + C
        \end{flalign*}
    \end{multicols}

    \begin{multicols}{2}
        \item $\displaystyle\int\dfrac{x^2 - 9}{x + 3}dx$
        \sol{}
        \begin{flalign*}
            I & = \int \dfrac{(x + 3)(x - 3)}{x + 3}dx & \\
              & = \int (x - 3)dx                       & \\
              & = \dfrac{1}{2}x^2 - 3x + C
        \end{flalign*}

        \item $\displaystyle\int\dfrac{x^3 - 8}{x - 2}dx$
        \sol{}
        \begin{flalign*}
            I & = \int \dfrac{(x - 2)(x^2 + 2x + 4)}{x - 2}dx & \\
              & = \int (x^2 + 2x + 4)dx                       & \\
              & = \dfrac{1}{3}x^3 + x^2 + 4x + C
        \end{flalign*}
    \end{multicols}

    \begin{multicols}{2}
        \item $\displaystyle\int\sqrt[3]{x^2}\left(\sqrt{x} - \dfrac{1}{x}\right)dx$
        \sol{}
        \begin{flalign*}
            I & = \int x^{\frac{2}{3}}\left(x^{\frac{1}{2}} - x^{-1}\right)dx     & \\
              & = \int \left(x^{\frac{7}{6}} - x^{-\frac{1}{3}}\right)dx          & \\
              & = \dfrac{6}{13}x^{\frac{13}{6}} - \dfrac{3}{2}x^{\frac{2}{3}} + C
        \end{flalign*}

        \item $\displaystyle\int\dfrac{(2x + 1)^2}{x}dx$
        \sol{}
        \begin{flalign*}
            I & = \int\dfrac{4x^2 + 4x + 1}{x}dx            & \\
              & = \int \left(4x + 4 + \dfrac{1}{x}\right)dx & \\
              & = 2x^2 + 4x + \ln|x| + C
        \end{flalign*}
    \end{multicols}

    \begin{multicols}{2}
        \item $\displaystyle\int\dfrac{(x + 1)(3x^2 - 4)}{2x^3}dx$
        \sol{}
        \begin{flalign*}
            I & = \int\dfrac{3x^3 + 3x^2 - 4x - 4}{2x^3}dx                                          & \\
              & = \int\left(\dfrac{3}{2} + \dfrac{3}{2x} - \dfrac{2}{x^2} - \dfrac{2}{x^3}\right)dx & \\
              & = \dfrac{3}{2}x - \dfrac{3}{2}\ln|x| + \dfrac{2}{x} + \dfrac{1}{x^2} + C
        \end{flalign*}
        \vfill{}\null{}

        \item $\displaystyle\int\left(\dfrac{x - 1}{x^2}\right)^2dx$
        \sol{}
        \begin{flalign*}
            I & = \int\left(\dfrac{x^2 - 2x + 1}{x^4}\right)dx         & \\
              & = \int\left(x^{-2} - 2x^{-3} + x^{-4}\right)dx         & \\
              & = -x^{-1} + x^{-2} - \dfrac{1}{3}x^{-3} + C            & \\
              & = -\dfrac{1}{x} + \dfrac{1}{x^2} - \dfrac{1}{3x^3} + C
        \end{flalign*}
    \end{multicols}

    \begin{multicols}{2}
        \item $\displaystyle\int\left(\sin\dfrac{x}{2} - \cos\dfrac{x}{2}\right)^2dx$
        \sol{}
        \begin{flalign*}
            I & = \int\left(\sin^2\dfrac{x}{2} - 2\sin\dfrac{x}{2}\cos\dfrac{x}{2} + \cos^2\dfrac{x}{2}\right)dx & \\
              & = \int\left(1 - \sin x\right)dx = x + \cos x + C
        \end{flalign*}
        \vfill{}\null{}

        \item $\displaystyle\int\tan^2xdx$
        \sol{}
        \begin{flalign*}
            I & = \int(\sec^2x - 1)dx & \\
              & = \tan x - x + C
        \end{flalign*}
        \vfill{}\null{}
    \end{multicols}
    \vspace{-3em}

    \begin{multicols}{2}
        \item $\displaystyle\int\left(e^2 + \dfrac{1}{4x}\right)dx$
        \sol{}
        \begin{flalign*}
            I & = \int e^2dx + \dfrac{1}{4}\int\dfrac{1}{x}dx & \\
              & = e^2x + \dfrac{1}{4}\ln|x| + C
        \end{flalign*}

        \item $\displaystyle\int(2e)^xdx$
        \sol{}
        \begin{flalign*}
            I & = \dfrac{(2e)^x}{\ln(2e)} + C   & \\
              & = \dfrac{(2e)^x}{\ln 2 + 1} + C
        \end{flalign*}
    \end{multicols}

    \begin{multicols}{2}
        \item Given the function $y = \dfrac{5x}{3 - x}$, find $\dfrac{dy}{dx}$. Hence,
        \\find $\displaystyle\int\dfrac{1}{(3 - x)^2}dx$. \sol{}
        \begin{flalign*}
            \dfrac{dy}{dx}             & = \dfrac{5(3 - x) - 5x(-1)}{(3 - x)^2}          & \\
                                       & = \dfrac{15}{(3 - x)^2}                         & \\
                                       &                                                   \\
            \int\dfrac{1}{(3 - x)^2}dx & = \int\dfrac{1}{15}\cdot\dfrac{15}{(3 - x)^2}dx & \\
                                       & = \dfrac{1}{15}\int\dfrac{15}{(3 - x)^2}dx      & \\
                                       & = \dfrac{1}{15}\int\dfrac{dy}{dx}dx             & \\
                                       & = \dfrac{1}{15}y + C                            & \\
                                       & = \dfrac{1}{15}\cdot\dfrac{5x}{3 - x} + C       & \\
                                       & = \dfrac{x}{3(3 - x)} + C
        \end{flalign*}

        \item If the function $y = \dfrac{2x^2}{3x - 1}$, find $\dfrac{dy}{dx}$. Hence,
        \\find $\displaystyle\int\dfrac{2x - 3x^2}{(3x - 1)^2}dx$. \sol{}
        \begin{flalign*}
            \dfrac{dy}{dx}                      & = \dfrac{2(3x - 1)(2x) - 2x^2(3)}{(3x - 1)^2}     & \\
                                                & = \dfrac{12x^2 - 4x - 6x^2}{(3x - 1)^2}           & \\
                                                & = \dfrac{6x^2 - 4x}{(3x - 1)^2}                   & \\
                                                &                                                     \\
            \int\dfrac{2x - 3x^2}{(3x - 1)^2}dx & = -dfrac{1}{2}\int\dfrac{6x^2 - 4x}{(3x - 1)^2}dx & \\
                                                & = -\dfrac{1}{2}\int\dfrac{dy}{dx}dx               & \\
                                                & = -\dfrac{1}{2}y + C                              & \\
                                                & = -\dfrac{1}{2}\cdot\dfrac{2x^2}{3x - 1} + C      & \\
                                                & = -\dfrac{x^2}{3x - 1} + C
        \end{flalign*}
    \end{multicols}

    \item Prove that $\dfrac{d}{dx}\left(\dfrac{3x^2}{x^2 + 2}\right) = \dfrac{12x}{(x^2
                  + 2)^2}$. Hence, find $\displaystyle\int\dfrac{4x}{(x^2 + 2)^2}dx$. \sol{}
          \begin{flalign*}
              \dfrac{d}{dx}\left(\dfrac{3x^2}{x^2 + 2}\right) & = \dfrac{(x^2 + 2)(6x) - (3x^2)(2x)}{(x^2 + 2)^2} & \\
                                                              & = \dfrac{6x^3 + 12x - 6x^3}{(x^2 + 2)^2}          & \\
                                                              & = \dfrac{12x}{(x^2 + 2)^2} \qquad \blacksquare
          \end{flalign*}
          \newpage{}

    \item Given that ${\dfrac{d}{dx}}{\left(\dfrac{3x^{2}-1}{5x^{2}+7}\right)}=f(x)$,
          find $\displaystyle\int\left[3x^2 - 1 - 2f(x)\right]dx$. \sol{}
          \begin{flalign*}
              \int\left[3x^2 - 1 - 2f(x)\right]dx & = \int3x^2dx - \int dx - 2\int f(x)dx            & \\
                                                  & = x^3 - x - 2\cdot\dfrac{3x^2 - 1}{5x^2 + 7} + C & \\
                                                  & = x^3 - x - \dfrac{6x^2 - 2}{5x^2 + 7} + C
          \end{flalign*}

    \item Given that ${\dfrac{d}{dx}}\left({\dfrac{2+x^{3}}{2-x^{3}}}\right)=3g(x)$, find
          $\displaystyle\int\left[g(x) - 3x + 2\right]dx$. \sol{}
          \begin{flalign*}
              \int\left[g(x) - 3x + 2\right]dx & = \int g(x)dx - 3\int xdx + 2\int dx                                           & \\
                                               & = \int g(x)dx - \dfrac{3}{2}x^2 + 2x + C                                       & \\
                                               & = \int\dfrac{1}{3}\cdot3g(x)dx - \dfrac{3}{2}x^2 + 2x + C                      & \\
                                               & = \dfrac{1}{3}\left(\dfrac{2 + x^3}{2 - x^3}\right) - \dfrac{3}{2}x^2 + 2x + C & \\
                                               & = \dfrac{2 + x^3}{3(2 - x^3)} - \dfrac{3}{2}x^2 + 2x + C
          \end{flalign*}
\end{enumerate}