\subsection{Practice 6}
Find the following indefinite integral:
\begin{enumerate}
    \begin{multicols}{2}
        \item $\displaystyle\int\dfrac{x}{(x-1)(x-2)} dx$
        \sol{}

        Let $\dfrac{x}{(x-1)(x-2)} = \dfrac{A}{x-1} + \dfrac{B}{x-2}$.
        \begin{flalign*}
            \dfrac{x}{(x-1)(x-2)} & = \dfrac{A}{x-1} + \dfrac{B}{x-2} & \\
            x                     & = Ax - 2A + Bx - B                & \\
                                  & = (A + B)x - (2A + B)
        \end{flalign*}
        \vspace{-2em}
        \begin{flalign*}
            \begin{cases}
                A + B = 1 \\
                2A + B = 0
            \end{cases}
            \Rightarrow
            \begin{cases}
                A = -1 \\
                B = 2
            \end{cases}
        \end{flalign*}
        \vspace{-1em}
        \begin{flalign*}
            I & = \int\left(\dfrac{-1}{x-1} + \dfrac{2}{x-2}\right) dx & \\
              & = 2\ln|x-2| - \ln|x-1| + C
        \end{flalign*}

        \columnbreak

        \item $\displaystyle\int\dfrac{x}{(x-1)^2} dx$
        \sol{}

        Let $u = x - 1$, $du = dx$, $x = u + 1$.
        \begin{flalign*}
            I & = \int\dfrac{u + 1}{u^2} du                 & \\
              & = \int\left(\dfrac{1}{u} + u^{-2}\right) du & \\
              & = \ln|u| - u^{-1} + C                       & \\
              & = \ln|x-1| - \dfrac{1}{x-1} + C
        \end{flalign*}
    \end{multicols}
\end{enumerate}