% chktex-file 2% chktex-file 29
% chktex-file 13
\documentclass{report}
\usepackage{setspace}
\usepackage[a4paper, total={7in, 9in}]{geometry}
\usepackage[fleqn]{amsmath}
\usepackage{empheq}
\usepackage{amssymb}
\usepackage{amsthm}
\usepackage{gensymb}
\usepackage[fleqn]{cases}
\usepackage{multicol}
\usepackage{color}
\usepackage{stix}
\usepackage{chngcntr}
\usepackage{tikz}
\usepackage{enumitem}
\usetikzlibrary{calc,matrix,arrows}

\counterwithout{equation}{chapter}
\setlength{\columnseprule}{1pt}
\setlength{\columnsep}{24pt}
\setcounter{chapter}{14}
\hfuzz=100pt

\newtheorem{theorem}{Theorem}

\begin{document}
\newcommand{\sol}[1]{

    \noindent \textbf{Sol.}
}
\newcommand{\prooff}[1]{

    \noindent \textbf{Proof.}
}
\newcommand\m[1]{\begin{pmatrix}#1\end{pmatrix}}
\newcommand\vm[1]{\begin{vmatrix}#1\end{vmatrix}}
\newenvironment{amatrix}[1]{%
    \left(\begin{array}{@{}*{#1}{c}|c@{}}
        }{%
    \end{array}\right)
}
\begin{titlepage}
    \raggedleft{}
    \rule{1pt}{\textheight}
    \hspace{0.02\textwidth}
    \parbox[b]{0.75\textwidth}{

    {\Huge\bfseries Solution Book of \\[0.5\baselineskip] Mathematic}\\[2\baselineskip]
    {\large\textit{Ssnior 2 Part I}}\\[4\baselineskip]
    {\Large\textsc{MELVIN CHIA}}

    \vspace{0.5\textheight}

    {\noindent Written on 9 October 2022}\\[\baselineskip]
    }

\end{titlepage}

\doublespacing{}
\tableofcontents
\singlespacing{}
\newpage

\begin{multicols}{2}

    \section{Fractional Inequalities}

    Inequalities that involve fractional expressions are called fractional
    inequalities. To solve a fractional inequality, we manipulate the inequality
    until the right side is zero.

    \subsection{Practice 8}

    Solve the following inequalities:

    \begin{enumerate}

        \item $\frac{x-5}{3x + 1} > 2$
              \sol{}
              \begin{flalign*}
                  \frac{x-5}{3x + 1}               & > 2            \\
                  \frac{x - 5}{3x + 1} - 2         & > 0            \\
                  \frac{x - 5 - 2(3x + 1)}{3x + 1} & > 0            \\
                  \frac{x - 5 - 6x - 2}{3x + 1}    & > 0            \\
                  \frac{-5x - 7}{3x + 1}           & > 0            \\
                  -\frac{5x + 7}{3x + 1}           & > 0            \\
                  \frac{5x + 7}{3x + 1}            & < 0            \\
                  -\frac{7}{5} < x                 & < -\frac{1}{3}
              \end{flalign*}
              \begin{center}
                  \begin{tikzpicture}
                      \draw[latex-latex] (0,0) -- (6,0);
                      \draw[shift={(2,0)},color=black] (0pt,3pt) -- (0pt,-3pt) node[below] {$-\frac{7}{5}$};
                      \draw[shift={(4,0)},color=black] (0pt,3pt) -- (0pt,-3pt) node[below] {$-\frac{1}{3}$};
                      \draw[shift={(1,0)},color=black] node[above] {$+$};
                      \draw[shift={(3,0)},color=black] node[above] {$-$};
                      \draw[shift={(5,0)},color=black] node[above] {$+$};
                      \node[circle,draw,fill=white,inner sep=1.5pt](a)at(2,1){};
                      \draw (a)--(4,1);
                      \node[circle,draw,fill=white,inner sep=1.5pt](b)at(4,1){};
                  \end{tikzpicture}
              \end{center}

        \item $\frac{x + 22}{x - 2} < x + 1$
              \sol{}
              \begin{flalign*}
                  \frac{x + 22}{x - 2}                  & < x + 1 \\
                  \frac{x + 22 - (x - 2)(x + 1)}{x - 2} & < 0     \\
                  \frac{x + 22 - x^2 + x + 2}{x - 2}    & < 0     \\
                  \frac{-x^2 + 2x + 24}{x - 2}          & < 0     \\
                  \frac{x^2 - 2x - 24}{x - 2}           & > 0     \\
                  \frac{(x - 6)(x + 4)}{x-2}            & > 0     \\
                  -4 < x < 2 \text{ or } x              & > 6
              \end{flalign*}
              \begin{center}
                  \begin{tikzpicture}
                      \draw[latex-latex] (0,0) -- (6,0);
                      \draw[shift={(1,0)},color=black] (0pt,3pt) -- (0pt,-3pt) node[below] {$-4$};
                      \draw[shift={(3,0)},color=black] (0pt,3pt) -- (0pt,-3pt) node[below] {$2$};
                      \draw[shift={(5,0)},color=black] (0pt,3pt) -- (0pt,-3pt) node[below] {$6$};
                      \draw[shift={(0.5,0)},color=black] node[above] {$-$};
                      \draw[shift={(2,0)},color=black] node[above] {$+$};
                      \draw[shift={(4,0)},color=black] node[above] {$-$};
                      \draw[shift={(5.5,0)},color=black] node[above] {$+$};
                      \node[circle,draw,fill=white,inner sep=1.5pt](a)at(1,1){};
                      \draw (a)--(3,1);
                      \node[circle,draw,fill=white,inner sep=1.5pt](b)at(3,1){};
                      \node[circle,draw,fill=white,inner sep=1.5pt](c)at(5,1){};
                      \draw[-latex,black] (c)--(6,1);
                  \end{tikzpicture}
              \end{center}

        \item $\frac{1}{x - 3} \geq \frac{1}{2x-1}$
              \sol{}
              \begin{flalign*}
                  \frac{1}{x - 3}                                   & \geq \frac{1}{2x-1}                          \\
                  \frac{2x - 1 - x + 3}{(x - 3)(2x - 1)}            & \geq 0                                       \\
                  \frac{x + 2}{(x - 3)(2x - 1)}                     & \geq 0                                       \\
                  \text{When } \frac{x + 2}{(x - 3)(2x - 1)}        & = 0,\ x = -2                                 \\
                  \text{When } \frac{x + 2}{(x - 3)(2x - 1)}        & > 0,\ -2 < x < \frac{1}{2} \text{ or } x > 3 \\
                  \therefore\ -2 \leq x < \frac{1}{2} \text{ or } x & > 3
              \end{flalign*}
              \begin{center}
                  \begin{tikzpicture}
                      \draw[latex-latex] (0,0) -- (6,0);
                      \draw[shift={(1,0)},color=black] (0pt,3pt) -- (0pt,-3pt) node[below] {$-2$};
                      \draw[shift={(3,0)},color=black] (0pt,3pt) -- (0pt,-3pt) node[below] {$\frac{1}{2}$};
                      \draw[shift={(5,0)},color=black] (0pt,3pt) -- (0pt,-3pt) node[below] {$3$};
                      \draw[shift={(0.5,0)},color=black] node[above] {$-$};
                      \draw[shift={(2,0)},color=black] node[above] {$+$};
                      \draw[shift={(4,0)},color=black] node[above] {$-$};
                      \draw[shift={(5.5,0)},color=black] node[above] {$+$};
                      \node[circle,draw,fill=white,inner sep=1.5pt](a)at(1,1){};
                      \draw (a)--(3,1);
                      \node[circle,draw,fill=white,inner sep=1.5pt](b)at(3,1){};
                      \node[circle,draw,fill=white,inner sep=1.5pt](c)at(5,1){};
                      \draw[-latex,black] (c)--(6,1);
                  \end{tikzpicture}
              \end{center}

        \item $\frac{x^2 - 7}{1 - x^2} \leq 1$
              \sol{}
              \begin{flalign*}
                  \frac{x^2 - 7}{1 - x^2}                            & \leq 1                                               \\
                  \frac{x^2 - 7 - 1 + x^2}{1 - x^2}                  & \leq 0                                               \\
                  \frac{2x^2 - 8}{(1 + x)(1-x)}                      & \leq 0                                               \\
                  \frac{2(x+2)(x-2)}{-(x+1)(x-1)}                    & \leq 0                                               \\
                  \frac{(x + 2)(x - 2)}{(x + 1)(x - 1)}              & \geq 0                                               \\
                  \text{When } \frac{(x + 2)(x - 2)}{(x + 1)(x - 1)} & = 0,\ x = -2 \text{ or } x = 2                       \\
                  \text{When } \frac{(x + 2)(x - 2)}{(x + 1)(x - 1)} & > 0,                                                 \\
                  x < -2 \text{ or } -1 < x                          & < 1                      \text{ or } x        > 2    \\
                  \therefore\ x \leq -2 \text{ or } -1 \leq x        & < 1                      \text{ or } x        \geq 2
              \end{flalign*}
              \begin{center}
                  \begin{tikzpicture}
                      \draw[latex-latex] (0,0) -- (7,0);
                      \draw[shift={(1,0)},color=black] (0pt,3pt) -- (0pt,-3pt) node[below] {$-2$};
                      \draw[shift={(3,0)},color=black] (0pt,3pt) -- (0pt,-3pt) node[below] {$-1$};
                      \draw[shift={(4,0)},color=black] (0pt,3pt) -- (0pt,-3pt) node[below] {$1$};
                      \draw[shift={(6,0)},color=black] (0pt,3pt) -- (0pt,-3pt) node[below] {$2$};
                      \draw[shift={(0.5,0)},color=black] node[above] {$+$};
                      \draw[shift={(2,0)},color=black] node[above] {$-$};
                      \draw[shift={(3.5,0)},color=black] node[above] {$+$};
                      \draw[shift={(5,0)},color=black] node[above] {$-$};
                      \draw[shift={(6.5,0)},color=black] node[above] {$+$};
                      \node[circle,draw,fill=white,inner sep=1.5pt](a)at(3,1){};
                      \draw (a)--(4,1);
                      \node[circle,draw,fill=white,inner sep=1.5pt](b)at(4,1){};
                      \node[circle,draw,fill=white,inner sep=1.5pt](c)at(6,1){};
                      \draw[-latex,black] (c)--(7,1);
                      \node[circle,draw,fill=white,inner sep=1.5pt](d)at(1,1){};
                      \draw[-latex,black] (d)--(0,1);
                  \end{tikzpicture}
              \end{center}

    \end{enumerate}

    \subsection{Exercise 15.5}

    Solve the following inequalities:

    \begin{enumerate}

        \item $\frac{7 - x}{9 - x} > \frac{1}{2}$
        \item $\frac{5 - x}{2} \geq \frac{3 - x}{x}$
        \item $\frac{x - 4}{x + 6} > \frac{1}{x}$
        \item $\frac{1}{x - 3} \geq \frac{1}{2x + 2}$
        \item $\frac{x - 1}{x + 1} - \frac{1}{x - 1} \leq 1$
        \item $1 + \frac{1}{x - 2} \leq \frac{x - 2}{x - 1}$
        \item $\frac{x^2 + x - 6}{x^2 + 4x + 4} \leq 0$
        \item $\frac{2x^2 - 3x + 1}{x^2 + 5x + 6} \geq 0$

    \end{enumerate}

\end{multicols}
\end{document}